chore: preparing for v2

Cvc/Basic.lean
@@ -1,525 +1,598 @@
 /-
-Copyright (c) 2023-2025 by the authors listed in the file AUTHORS and their
+Copyright (c) 2025 by the authors listed in the file AUTHORS and their
 institutional affiliations. All rights reserved.
 Released under Apache 2.0 license as described in the file LICENSE.
 Authors: Adrien Champion
 -/
 
-import Batteries.Data.Rat.Basic
-import Batteries.Data.RBMap
+module
 
-import cvc5
+public meta import Lean.Elab.Command
 
+public import Cvc.Basic.Basic
+public import Cvc.Basic.Error
+public import Cvc.Basic.Env
 
-
-/-! # Library setup: re-exports and helpers -/
-namespace Cvc
-
-
-
-/-- The constant combinator. -/
-abbrev 𝕂 (val : α) (_ : β) : α := val
+import all Cvc.Basic.Env
 
 
-abbrev RBMap (α β : Type) [Ord α] :=
-  Batteries.RBMap α β compare
 
-namespace RBMap variable [Ord α]
+namespace Cvc -- variable [Ω]
 
-open Batteries renaming RBMap → Map
+section open Lean Elab Command
 
-/-- The empty map. -/
-def empty : RBMap α β := Map.empty
+syntax (name := enumDefStx)
+  atomic( (docComment)? "enum_def%") ident " ← " ("[" ident "/" ident "]")? ident
+    (ppLine ppIndent(
+      atomic((docComment ppLine)? "| ") ("default!")? rawIdent " ← " ident
+    ))*
+: command
 
-/-- Builds a map from a list. -/
-def ofList : List (α × β) → RBMap α β :=
-  (Map.ofList · compare)
+open Parser.Term (attrInstance) in
+@[command_elab enumDefStx]
+public meta def enumDefStxElab : CommandElab
+| `(
+  $[ $doc?:docComment ]?
+  enum_def% $id  ← $[[$ofSrcId? / $toSrcId?]]? $srcId
+    $[ $[ $variantDocs?:docComment ]?
+    | $[ default!%$default? ]? $variantIds ← $variantSrcIds ]*
+) => do
+  let ofSrcId ← ofSrcId?.getDM do `ofUnsafe |> mkIdent |> pure
+  let toSrcId ← toSrcId?.getDM do `toUnsafe |> mkIdent |> pure
+  let variantDefault? := default?.zip variantIds |>.find? (Option.isSome ∘ Prod.fst) |>.map Prod.snd
+  let variantSrcIds := variantSrcIds.map (· |>.getId |> srcId.getId.append |> mkIdent)
+  let mods ←
+    if let some doc := doc? then `(declModifiers| $doc:docComment)
+    else `(declModifiers| @[inherit_doc $srcId])
+  let stx ← `(
+      $mods:declModifiers
+      inductive $id:ident where
+      $[ $[ $variantDocs?:docComment ]? | $variantIds:ident ]*
+      deriving Repr, BEq, DecidableEq, Hashable, Ord
+    )
+  elabCommand stx
 
-/-- Removes from `map` the bindings `key`/`val` such that `¬ f key val`. -/
-def filter : (map : RBMap α β) → (f : α → β → Bool) → RBMap α β :=
-  Map.filter
+  let leanDefaultId := ``default |> mkIdent
+  let leanReprId := ``repr |> mkIdent
+  let leanToStringId := ``toString |> mkIdent
+  let defaultDef ←
+    if let some variantDefault := variantDefault? then `($variantDefault:ident)
+    else `( .ofNat 0 )
+  let propOfTo := s!"{ofSrcId.getId}_{toSrcId.getId}" |> Name.mkStr1 |> mkIdent
+  let propToOf := s!"{toSrcId.getId}_{ofSrcId.getId}" |> Name.mkStr1 |> mkIdent
+  let bleId := `ble |> mkIdent
+  let bltId := `blt |> mkIdent
+  let stx ← `(
+    namespace $id
+    /-- Translation from cvc5. -/
+    private def $ofSrcId:ident (val : $srcId) : $id := val.ctorIdx |> .ofNat
+    /-- Translation to cvc5. -/
+    private def $toSrcId:ident (val : $id) : $srcId := val.ctorIdx |> .ofNat
+    private theorem $propOfTo:ident (val : $id) : $ofSrcId ($toSrcId val) = val :=
+      by cases val <;> rfl
+    private theorem $propToOf (val : $srcId) : $toSrcId ($ofSrcId val) = val :=
+      by cases val <;> rfl
 
-/-- Removes from `map` the bindings `key`/`val` such that `¬ f val`. -/
-def filterVal (map : RBMap α β) (f : β → Bool) : RBMap α β :=
-  map.filter fun _ => f
+    instance : Inhabited $id := ⟨$defaultDef⟩
+    /-- Default value. -/
+    protected def default : $id := $leanDefaultId
 
-/-- Inserts a `key`/`val` binding in a map.
+    instance : ToString $id := ⟨(s!"{$leanReprId ·}")⟩
+    /-- String representation. -/
+    protected def toString : $id → String := $leanToStringId
 
-See also `RBMap.insert'`.
+    protected abbrev $bleId (val1 val2 : $id) : Bool :=
+      match compare val1 val2 with | Ordering.lt | Ordering.eq => true | Ordering.gt => false
+    instance : LE $id := ⟨(· |>.$bleId ·)⟩
+    instance : DecidableLE $id :=
+      fun val1 val2 => if h : val1 |>.$bleId val2 then isTrue h else isFalse h
+
+    protected abbrev $bltId (val1 val2 : $id) : Bool :=
+      match compare val1 val2 with | Ordering.lt => true | Ordering.eq | Ordering.gt => false
+    instance : LT $id := ⟨(· |>.$bltId ·)⟩
+    instance : DecidableLT $id :=
+      fun val1 val2 => if h : val1 |>.$bltId val2 then isTrue h else isFalse h
+    end $id
+  )
+  elabCommand stx
+
+  for (variantId, variantSrcId) in variantIds.zip variantSrcIds do
+    let stx ←
+      `(open $id:ident in example : ($toSrcId:ident $variantId:ident) = $variantSrcId:ident := rfl)
+    elabCommand stx
+    let stx ←
+      `(open $id:ident in example : ($ofSrcId:ident $variantSrcId:ident) = $variantId:ident := rfl)
+    elabCommand stx
+| _ => throwUnsupportedSyntax
+
+
+public section
+
+enum_def% Unknown.Explanation ← cvc5.UnknownExplanation
+  | requiresFullCheck ← REQUIRES_FULL_CHECK
+  | incomplete ← INCOMPLETE
+  | timeOut ← TIMEOUT
+  | resourceOut ← RESOURCEOUT
+  | memOut ← MEMOUT
+  | interrupted ← INTERRUPTED
+  | unsupported ← UNSUPPORTED
+  | other ← OTHER
+  | requiresCheckAgain ← REQUIRES_CHECK_AGAIN
+  | default! unknownReason ← UNKNOWN_REASON
+
+enum_def% Float.RoundingMode ← cvc5.RoundingMode
+  | nearestTiesToEven ← ROUND_NEAREST_TIES_TO_EVEN
+  | towardPositive ← ROUND_TOWARD_POSITIVE
+  | towardNegative ← ROUND_TOWARD_NEGATIVE
+  | towardZero ← ROUND_TOWARD_ZERO
+  | nearestTiesToAway ← ROUND_NEAREST_TIES_TO_AWAY
+
+enum_def% Model.BlockMode ← cvc5.BlockModelsMode
+  /-- Block models based on the SAT skeleton. -/
+  | literals ← LITERALS
+  /-- Block models based on the concrete model values for the free variables. -/
+  | values ← VALUES
+
+/-- Types of learned literals.
+
+Note that a literal may conceptually belong to multiple categories. We
+classify literals based on the first criteria in this list that they meet.
 -/
-def insert : (map : RBMap α β) → (key : α) → (val : β) → RBMap α β :=
-  Map.insert
+enum_def% LearnedLitType ← cvc5.LearnedLitType
+  /-- An equality that was turned into a substitution during preprocessing.
 
-/-- Adds a `key`/`val` binding in a map, returns the previous value of `key` if any.
+  In particular, literals in this category are of the form (= x t) where
+  x does not occur in t.
+  -/
+  | preprocessSolved ← PREPROCESS_SOLVED
+  /-- A top-level literal (unit clause) from the preprocessed set of input formulas. -/
+  | preprocess ← PREPROCESS
+  /--
+  A literal from the preprocessed set of input formulas that does not
+  occur at top-level after preprocessing.
 
-See also `RBMap.insert`.
+  Typically, this is the most interesting category of literals to learn.
+  -/
+  | input ← INPUT
+  /-- An internal literal that is solvable for an input variable.
+
+  In particular, literals in this category are of the form (= x t) where
+  x does not occur in t, the preprocessed set of input formulas contains the
+  term x, but not the literal (= x t).
+
+  Note that solvable literals can be turned into substitutions during
+  preprocessing.
+  -/
+  | solvable ← SOLVABLE
+  /-- An internal literal that can be made into a constant propagation for an input term.
+
+  In particular, literals in this category are of the form (= t c) where
+  c is a constant, the preprocessed set of input formulas contains the
+  term t, but not the literal (= t c).
+  -/
+  | constantProp ← CONSTANT_PROP
+  /-- Any internal literal that does not fall into the above categories. -/
+  | internal ← INTERNAL
+  /-- Special case for when produce-learned-literals is not set. -/
+  | unknown ← UNKNOWN
+
+enum_def% Proof.Component ← cvc5.ProofComponent
+  | rawPreprocess ← RAW_PREPROCESS
+  | preprocess ← PREPROCESS
+  | sat ← SAT
+  | theoryLemmas ← THEORY_LEMMAS
+  | default! full ← FULL
+
+enum_def% Proof.Format ← cvc5.ProofFormat
+  | no ← NONE
+  | dot ← DOT
+  | lfsc ← LFSC
+  | alethe ← ALETHE
+  | cpc ← CPC
+  | default! fromSolver ← DEFAULT
+
+
+
+/--
+Find synthesis targets, used as an argument to Solver::findSynth. These
+specify various kinds of terms that can be found by this method.
 -/
-def insert' (map : RBMap α β) (key : α) (val : β) : (Option β) × RBMap α β :=
-  (map.find? key, map.insert key val)
+enum_def% Synth.FindTarget ← cvc5.FindSynthTarget
+  /--
+  Find the next term in the enumeration of the target grammar.
+  -/
+  | enum ← ENUM
+  /--
+  Find a pair of terms (t,s) in the target grammar which are equivalent
+  but do not rewrite to the same term in the given rewriter
+  (--sygus-rewrite=MODE). If so, the equality (= t s) is returned by
+  findSynth.
 
-/-- Adds a `key`/`val` binding in a map, `none` if a binding for `key` already exists. -/
-def insertNew? (map : RBMap α β) (key : α) (val : β) : Option (RBMap α β) :=
-  let (prev?, map) := map.insert' key val
-  prev?.map (𝕂 map)
+  This can be used to synthesize rewrite rules. Note if the rewriter is set
+  to none (--sygus-rewrite=none), this indicates a possible rewrite when
+  implementing a rewriter from scratch.
+  -/
+  | rewrite ← REWRITE
+  /--
+  Find a term t in the target grammar which rewrites to a term s that is
+  not equivalent to it. If so, the equality (= t s) is returned by
+  findSynth.
 
-/-- Removes from `map` the binding for `key`, if any.
+  This can be used to test the correctness of the given rewriter. Any
+  returned rewrite indicates an unsoundness in the given rewriter.
+  -/
+  | rewriteUnsound ← REWRITE_UNSOUND
+  /--
+  Find a rewrite between pairs of terms (t,s) that are matchable with terms
+  in the input assertions where t and s are equivalent but do not rewrite
+  to the same term in the given rewriter (--sygus-rewrite=MODE).
 
-See also `RBMap.erase'`.
+  This can be used to synthesize rewrite rules that apply to the current
+  problem.
+  -/
+  | rewriteInput ← REWRITE_INPUT
+  /--
+  Find a query over the given grammar. If the given grammar generates terms
+  that are not Boolean, we consider equalities over terms from the given
+  grammar.
+
+  The algorithm for determining which queries to generate is configured by
+  --sygus-query-gen=MODE. Queries that are internally solved can be
+  filtered by the option --sygus-query-gen-filter-solved.
+  -/
+  | query ← QUERY
+
+/-- Option category enumeration.
+
+Specifies the category of an option for user interface purposes.
 -/
-def erase : (map : RBMap α β) → (key : α) → RBMap α β :=
-  Map.erase
-
-/-- Removes a `key`/`val` binding from a map, yields `some val` if such a binding existed.
-
-See also `RBMap.erase`.
--/
-def erase' (map : RBMap α β) (key : α) : (Option β) × RBMap α β :=
-  (map.find? key, map.erase key)
-
-/-- Removes a `key`/`val` binding from a map, `none` if no binding for `key` existed. -/
-def eraseExisting? (map : RBMap α β) (key : α) : Option (RBMap α β) :=
-  match map.erase' key with
-  | (some _, map) => map
-  | (none, _) => none
-
-/-- Map over the values of a map. -/
-def mapVal : (f : α → β → γ) → (map : RBMap α β) → RBMap α γ :=
-  Map.mapVal
-
-/-- Monadic filter/map over the values of a map. -/
-def filterMapValM [Monad m] (f : α → β → m (Option γ)) (map : RBMap α β) : m (RBMap α γ) :=
-  RBMap.empty |> map.foldlM fun map key val => do
-    if let some val ← f key val then return map.insert key val else return map
-
-/-- Monadic map over the values of a map. -/
-def mapValM [Monad m] (f : α → β → m γ) (map : RBMap α β) : m (RBMap α γ) :=
-  map.filterMapValM (some <$> f · ·)
-
-/-- Filter/map over the values of a map. -/
-def filterMapVal (f : α → β → Option γ) (map : RBMap α β) : RBMap α γ :=
-  map.filterMapValM (m := Id) f
-
-/-- Monadic filter/map over the values of a map into an array of values. -/
-def filterMapValToArrayM [Monad m] (f : α → β → m (Option γ)) (map : RBMap α β) : m (Array γ) :=
-  #[] |> map.foldlM fun array key val => do
-    if let some val ← f key val then return array.push val else return array
-
-/-- Filter/map over the values of a map into an array of values. -/
-def filterMapValToArray (f : α → β → Option γ) (map : RBMap α β) : Array γ :=
-  map.filterMapValToArrayM (m := Id) f
-
-/-- Monadic map over the values of a map into an array of values. -/
-def mapValToArrayM [Monad m] (f : α → β → m γ) (map : RBMap α β) : m (Array γ) :=
-  map.filterMapValToArrayM (some <$> f · ·)
-
-/-- Map over the values of a map into an array of values. -/
-def mapValToArray (f : α → β → γ) (map : RBMap α β) : Array γ :=
-  map.mapValToArrayM (m := Id) f
-
-/-- Monadic key-ignoring map over the values of a map. -/
-def mapOnlyValM [Monad m] (f : β → m γ) (map : RBMap α β) : m (RBMap α γ) :=
-  map.mapValM fun _ => f
-
-/-- Key-ignoring map over the values of a map. -/
-def mapOnlyVal (f : β → γ) (map : RBMap α β) : RBMap α γ :=
-  map.mapVal fun _ => f
-
-/-- Key-ignoring monadic filter/map over the values of a map. -/
-def filterMapOnlyValM [Monad m] (f : β → m (Option γ)) (map : RBMap α β) : m (RBMap α γ) :=
-  map.filterMapValM fun _ => f
-
-/-- Key-ignoring filter/map over the values of a map. -/
-def filterMapOnlyVal (f : β → Option γ) (map : RBMap α β) : RBMap α γ :=
-  map.filterMapOnlyValM (m := Id) f
-
-/-- Key-ignoring filter/map over the values of a map into an array of values. -/
-def filterMapOnlyValToArrayM [Monad m] (f : β → m (Option γ)) (map : RBMap α β) : m (Array γ) :=
-  map.filterMapValToArrayM fun _ => f
-
-/-- Key-ignoring filter/map over the values of a map into an array of values. -/
-def filterMapOnlyValToArray (f : β → Option γ) (map : RBMap α β) : Array γ :=
-  map.filterMapOnlyValToArrayM (m := Id) f
-
-/-- Key-ignoring monadic map over the values of a map into an array of values. -/
-def mapOnlyValToArrayM [Monad m] (f : β → m γ) (map : RBMap α β) : m (Array γ) :=
-  map.mapValToArrayM fun _ => f
-
-/-- Key-ignoring map over the values of a map into an array of values. -/
-def mapOnlyValToArray (f : β → γ) (map : RBMap α β) : Array γ :=
-  map.mapOnlyValToArrayM (m := Id) f
-
-def filterMapFoldM {Acc : Type} [Monad m] (init : Acc)
-  (f : Acc → α → β → m (Acc × Option γ))
-  (map : RBMap α β)
-: m (Acc × RBMap α γ) := do
-  let mut map' : RBMap α γ := .empty
-  let mut acc := init
-  for (key, val) in map do
-    let (acc', val?) ← f acc key val
-    acc := acc'
-    if let some val := val? then
-      map' := map'.insert key val
-  return (acc, map')
-
-
-end RBMap
-
-
-
-abbrev RBSet (α : Type) [Ord α] :=
-  Batteries.RBSet α compare
-
-namespace RBSet variable [Ord α]
-
-open Batteries renaming RBSet → Set
-
-/-- The empty set. -/
-def empty : RBSet α := Set.empty
-
-/-- Removes from `set` the elements `elm` for which `¬ f elm`. -/
-def filter : (set : RBSet α) → (f : α → Bool) → RBSet α :=
-  Set.filter
-
-/-- Inserts an element in the set.
-
-See also `RBSet.insert'`.
--/
-def insert : (set : RBSet α) → α → RBSet α :=
-  Set.insert
-
-/-- Inserts an element in the set, yields `true` *iff* the element is new.
-
-See also `RBSet.insert`.
--/
-def insert' (set : RBSet α) (elm : α) : Bool × RBSet α :=
-  (set.contains elm, set.insert elm)
-
-/-- Removes an element from a set.
-
-See also `RBSet.erase'`.
--/
-def erase (set : RBSet α) (k : α) : RBSet α := Set.erase set (compare k)
-
-/-- Removes an element from a set, yields `true` *iff* the element was there.
-
-See also `RBSet.erase`
--/
-def erase' (set : RBSet α) (elm : α) : Bool × RBSet α :=
-  (set.contains elm, set.insert elm)
-
-end RBSet
-
-
-
-def Decidable.conj {p q : Prop} [Decidable p] [Decidable q] : Decidable (p ∧ q) :=
-  inferInstance
-
-def Decidable.conj' {p q : Prop} (ip : Decidable p) (iq : Decidable q) : Decidable (p ∧ q) :=
-  inferInstance
-
-
-
-scoped
-syntax:max "ls!" interpolatedStr(term) : term
-macro_rules
-| `(ls! $interpSrt) => `( (fun () => s!$interpSrt : Unit → String)  )
-
-
-
-export _root_ (Rat)
-
-
-
-/-- A check-sat result.-/
-inductive CheckSat
-/-- Formulas asserted are satisfiable, *i.e.* a model exists. -/
-| sat
-/-- Formulas are unsatisfiable, no assignment of the symbols makes them true. -/
-| unsat
-/-- Solver returned unknown. -/
-| unknown (desc : String)
-/-- Solver returned some unexpected result. -/
-| other (desc : String)
-
-namespace CheckSat
-
-/-- Conversion to a simple *is sat?* flag, `none` on unknown/unexpected results. -/
-def isSat? : CheckSat → Option Bool
-| sat => true
-| unsat => false
-| unknown _ | other _ => none
-
-end CheckSat
-
-
-
-inductive Error : Type
-| internal (msg : String)
-| unsupported (msg : String)
-| userError (msg : String)
-deriving Inhabited
-
-
-namespace Error
-
-/-- Used to allow `String` and `Unit → String` as context messages. -/
-class AsString (α : Type) : Type where
-  /-- Conversion to strings. -/
-  asString : α → String
-
-instance : AsString String := ⟨id⟩
-instance : AsString (Unit → String) := ⟨fun f => f ()⟩
-
-def mapMsg (f : String → String) : Error → Error
-| .internal msg => f msg |> .internal
-| .unsupported msg => f msg |> .unsupported
-| .userError msg => f msg |> .userError
-
-def append (self : Error) (txt : String) (newline := true) : Error :=
-  let txt := if newline then "\n"++txt else txt
-  self.mapMsg (· ++ txt)
-
-
-def toCvc5 : Error → cvc5.Error
-| .internal "a value is missing" => .missingValue
-| .internal msg => .error msg
-| .unsupported msg => .unsupported msg
-| .userError msg => .error msg
-
-def ofCvc5 : cvc5.Error → Error
-| .missingValue => .internal "a value is missing"
-| .error msg => .internal s!"{msg}"
-| .option msg => .internal s!"option error: {msg}"
-| .unsupported msg => .unsupported msg
-| .recoverable msg => .internal s!"recoverable: {msg}"
-
-instance : MonadLift (Except cvc5.Error) (Except Error) where
-  monadLift
-  | .ok res => .ok res
-  | .error e => .error (ofCvc5 e)
-
-instance : Coe cvc5.Error Error := ⟨ofCvc5⟩
-
-protected def toString : Error → String
-| .internal msg => "internal error: " ++ msg
-| .unsupported msg => "unsupported: " ++ msg
-| .userError msg => "user error: " ++ msg
-
-instance instToString : ToString Error :=
-  ⟨Error.toString⟩
-
-section variable [Monad m] [MonadExcept Error m] (msg : String)
-
-/-- Throws an `Error.userError`. -/
-protected def throwUser : m α := do
-  throw <| Error.userError msg
-
-/-- Throws an `Error.internal`. -/
-protected def throwInternal : m α := do
-  throw <| Error.internal msg
-
-/-- Throws an `Error.internal` about unreachable code. -/
-protected def throwUnreachable (msg : String := "") : m α := do
-  let sep := if msg.isEmpty then "" else ": "
-  throw <| Error.internal s!"reached unreachable code{sep}{msg}"
+enum_def% Option.Category ← cvc5.OptionCategory
+  /-- Option available to regular users. -/
+  | regular ← REGULAR
+  /-- Option available to expert users. -/
+  | expert ← EXPERT
+  /-- Common options. -/
+  | common ← COMMON
+  /-- Undocumented options. -/
+  | undocumented ← UNDOCUMENTED
+
+/-- The different reasons for returning an "unknown" result. -/
+enum_def% InputLanguage ← cvc5.InputLanguage
+  /-- The SMT-LIB version 2.6 language. -/
+  | smtLib_2_6 ← SMT_LIB_2_6
+  /-- The SyGuS version 2.1 language. -/
+  | sygus_2_1 ← SYGUS_2_1
+  /-- No language given. -/
+  | unknown ← UNKNOWN
 
 end
 
-end Error
-
-export Error (throwUser throwInternal throwUnreachable)
 
 
 
-abbrev ResT m := ExceptT Error m
+-- inductive Term.Kind
+-- | uninterpretedSortValue
+-- | equal
+-- | distinct
+-- | const
+-- | var
+-- | skolem
+-- | sExpr
+-- | lambda
+-- | witness
+-- | boolConst
+-- | not
+-- | and
+-- | implies
+-- | or
+-- | xor
+-- | ite
+-- | apply_uf
+-- | cardinalityConstraint
+-- | hoApply
+-- | add
+-- | mult
+-- | iAnd
+-- | pIAnd
+-- | pow2
+-- | log2
+-- | sub
+-- | neg
+-- | div
+-- | divTotal
+-- | iDiv
+-- | iIdVTotal
+-- | iMod
+-- | iModTotal
+-- | abs
+-- | pow
+-- | exp
+-- | sine
+-- | cosine
+-- | tangent
+-- | coSecant
+-- | secant
+-- | coTangent
+-- | arcSine
+-- | arcCosine
+-- | arcTangent
+-- | arcCoSecant
+-- | arcSecant
+-- | arcCoTangent
+-- | sqrt
+-- | divisible
+-- | ratConst
+-- | intConst
+-- | lt
+-- | le
+-- | gt
+-- | ge
+-- | isInt
+-- | toInt
+-- | toReal
+-- | pi
+-- | constBv
+-- | bvConcat
+-- | bvAnd
+-- | bvOr
+-- | bvXor
+-- | bvNot
+-- | bvNAnd
+-- | bvNOr
+-- | bvXNOr
+-- | bvComp
+-- | bvMult
+-- | bvAdd
+-- | bvSub
+-- | bvNeg
+-- | bvUDiv
+-- | bvURem
+-- | bvSDiv
+-- | bvSRem
+-- | bvSMod
+-- | bvShl
+-- | bvLShr
+-- | bvAShr
+-- | bvULt
+-- | bvULe
+-- | bvUGt
+-- | bvUGe
+-- | bvSLt
+-- | bvSLe
+-- | bvSGt
+-- | bvSGe
+-- | bvULtBv
+-- | bvSLtBv
+-- | bvIte
+-- | bvRedOr
+-- | bvRedAnd
+-- | bvNegO
+-- | bvUAddO
+-- | bvSAddO
+-- | bvUMulO
+-- | bvSMulO
+-- | bvUSubO
+-- | bvSSubO
+-- | bvSDivO
+-- | bvExtract
+-- | bvRepeat
+-- | bvZeroExtend
+-- | bvSignExtend
+-- | bvRotateLeft
+-- | bvRotateRight
+-- | intToBv
+-- | bvToNat
+-- | bvUToInt
+-- | bvSToInt
+-- | bvFromBools
+-- | bvBit
+-- | finiteFieldConst
+-- | finiteFieldNeg
+-- | finiteFieldAdd
+-- | finiteFieldBitSum
+-- | finiteFieldMult
+-- | fpConst
+-- | roundingModeConst
+-- | fpOfBvs
+-- | fpEq
+-- | fpAbs
+-- | fpNeg
+-- | fpAdd
+-- | fpSub
+-- | fpMult
+-- | fpDiv
+-- | fpFma
+-- | fpSqrt
+-- | fpRem
+-- | fpRti
+-- | fpMin
+-- | fpMax
+-- | fpLe
+-- | fpLt
+-- | fpGe
+-- | fpGt
+-- | fpIsNormal
+-- | fpIsSubnormal
+-- | fpIsZero
+-- | fpIsInf
+-- | fpIsNan
+-- | fpIsNeg
+-- | fpIsPos
+-- | fpOfIeeeBv
+-- | fpOfFp
+-- | fpOfReal
+-- | fpOfSBv
+-- | fpOfUBv
+-- | fpToUBv
+-- | fpToSBv
+-- | fpToReal
+-- | arraySelect
+-- | arrayStore
+-- | arrayConst
+-- | arrayEqRange
+-- | dtApplyConstructor
+-- | dtApplySelector
+-- | dtApplyTester
+-- | dtApplyUpdater
+-- | patMatch
+-- | patMatchCase
+-- | patMatchBindCase
+-- | tupleProject
+-- | nullableLift
+-- | sepNil
+-- | sepEmp
+-- | sepPTo
+-- | sepStar
+-- | sepWand
+-- | setEmpty
+-- | setUnion
+-- | setInter
+-- | setMinus
+-- | setSubset
+-- | setMember
+-- | setSingleton
+-- | setInsert
+-- | setCard
+-- | setComplement
+-- | setUniverse
+-- | setComprehension
+-- | setChoose
+-- | setIsEmpty
+-- | setIsSingleton
+-- | setMap
+-- | setFilter
+-- | setAll
+-- | setAny
+-- | setFold
+-- | relationJoin
+-- | relationTableJoin
+-- | relationProduct
+-- | relationTranspose
+-- | relationTClosure
+-- | relationJoinImage
+-- | relationId
+-- | relationGroup
+-- | relationAggregate
+-- | relationProject
+-- | bagEmpty
+-- | bagUnionMax
+-- | bagUnionDisjoint
+-- | bagInterMin
+-- | bagDifferenceSubtract
+-- | bagDifferenceRemove
+-- | bagSubBag
+-- | bagCount
+-- | bagMember
+-- | bagToSet
+-- | bagMake
+-- | bagCard
+-- | bagChoose
+-- | bagMap
+-- | bagFilter
+-- | bagAll
+-- | bagAny
+-- | bagFold
+-- | bagPartition
+-- | tableProduct
+-- | tableProject
+-- | tableAggregate
+-- | tableJoin
+-- | tableGroup
+-- | stringConcat
+-- | stringInRegex
+-- | stringLength
+-- | stringSubstring
+-- | stringUpdate
+-- | stringCharAt
+-- | stringContains
+-- | stringIndexOf
+-- | stringIndexOfRegex
+-- | stringReplaceOne
+-- | stringReplaceAll
+-- | stringReplaceRegexOne
+-- | stringReplaceRegexAll
+-- | stringToLower
+-- | stringToUpper
+-- | stringRev
+-- | stringToCode
+-- | stringOfCode
+-- | stringLt
+-- | stringLe
+-- | stringPrefix
+-- | stringSuffix
+-- | stringIsDigit
+-- | stringOfInt
+-- | stringToInt
+-- | stringConst
+-- | stringToRegex
+-- | regexConcat
+-- | regexUnion
+-- | regexInter
+-- | regexDiff
+-- | regexStar
+-- | regexPlus
+-- | regexOpt
+-- | regexRange
+-- | regexRepeat
+-- | regexLoop
+-- | regexNone
+-- | regexAll
+-- | regexAllChar
+-- | regexComplement
+-- | seqConcat
+-- | seqLength
+-- | seqExtract
+-- | seqUpdate
+-- | seqAt
+-- | seqContains
+-- | seqIndexOf
+-- | seqReplaceOne
+-- | seqReplaceAll
+-- | seqRev
+-- | seqPrefix
+-- | seqSuffix
+-- | seqConst
+-- | seqUnit
+-- | seqNth
+-- | forall
+-- | exists
+-- | varList
+-- | instPattern
+-- | instNoPattern
+-- | instPool
+-- | instAddToPool
+-- | skolemAddToPool
+-- | instAttribute
+-- | instPatternList
+-- deriving Inhabited, BEq, DecidableEq, Ord, Hashable
 
-abbrev ResIO := ResT IO
+-- namespace Term.Kind open cvc5 renaming Kind → K
 
-/-- `Error`-result monad. -/
-abbrev Res := ResT Id
+-- section variable (k : Kind)
 
-namespace Res
-@[inherit_doc Except.ok]
-abbrev ok : α → Res α := Except.ok
-@[inherit_doc Except.error]
-abbrev error : Error → Res α := Except.error
+-- /-- Lower-bound of `cvc5.Kind` indices supported. -/
+-- private def idxLb := 3
+-- /-- Upper-bound of `cvc5.Kind` indices supported. -/
+-- private def idxUb := K.LAST_KIND.ctorIdx.pred
 
-instance : MonadLift (Except cvc5.Error) Res :=
-  ⟨fun | .ok v => .ok v | .error e => .error (Error.ofCvc5 e)⟩
+-- private def toUnsafe : K := K.ofNat (k.ctorIdx + idxLb)
 
-instance : MonadLift (Except cvc5.Error) Res :=
-  ⟨fun | .ok v => .ok v | .error e => .error (Error.ofCvc5 e)⟩
+-- private def ofUnsafe (k : K) : Res Kind :=
+--   let idx := k.ctorIdx
+--   if idxLb ≤ idx then
+--     if idx ≤ idxUb then return Kind.ofNat (k.ctorIdx - idxLb)
+--     else throwInternal s!"cannot convert above-range `cvc5.Kind` {k} to `Cvc.Kind`"
+--   else throwInternal s!"cannot convert below-range `cvc5.Kind` {k} to `Cvc.Kind`"
 
-instance [Monad m] : MonadLift Res (ResT m) := ⟨pure⟩
-
-def fail (e : Error) : Res α :=
-  .error e
-def failInternal (e : String) : Res α :=
-  Except.error.{0} <| .internal e
-def failUser (e : String) : Res α :=
-  Except.error.{0} <| .userError e
-def failTodo (e : String) : Res α :=
-  Except.error.{0} <| .unsupported e
-
-def context [A : Error.AsString S] (s : S) : Res α → Res α
-| .ok val => .ok val
-| .error e => .error <| e.mapMsg (s!"{·}\n{A.asString s}")
-
-def lift : Except cvc5.Error α → Res α := liftM
-
-end Res
-
-
-/-! ## Helpers -/
+-- end
 
 
 
-structure ArrayMin (n : Nat) (α : Type u) : Type u where
-mk' ::
-  pref : Array α
-  inv : pref.size = n := by rfl
-  suff : Array α := #[]
-deriving Hashable
+-- section tests
 
-namespace ArrayMin
+-- private example : uninterpretedSortValue.toUnsafe = K.UNINTERPRETED_SORT_VALUE := rfl
+-- private example : instPatternList.toUnsafe = K.INST_PATTERN_LIST := rfl
 
-instance [Inhabited α] : Inhabited (ArrayMin n α) where
-  default := ⟨Array.replicate n default, by simp, #[]⟩
+-- end tests
 
-def mk (pref : Array α) (suff : Array α := #[]) : ArrayMin pref.size α :=
-  ⟨pref, rfl, suff⟩
-
-protected def toString [ToString α] (self : ArrayMin n α) : String :=
-  if self.suff.isEmpty then
-    toString self.pref
-  else
-    s!"{self.pref}{self.suff}"
-
-instance [ToString α] : ToString (ArrayMin n α) := ⟨ArrayMin.toString⟩
-
-
-variable (self : ArrayMin n α)
-
-@[simp]
-theorem pref_size : self.pref.size = n :=
-  self.inv
-
-abbrev size : Nat := n + self.suff.size
-
-@[simp]
-theorem min_le_size : n ≤ self.size := by
-  simp only [Nat.le_add_right]
-
-def get : (i : Fin self.size) → α
-| ⟨i, h_i⟩ =>
-  if h : i < n then
-    have := self.pref_size ▸ h
-    self.pref[i]
-  else
-    have : i - n < self.suff.size := by
-      simp only [size] at h_i
-      exact Nat.sub_lt_left_of_lt_add (Nat.le_of_not_lt h) h_i
-    self.suff[i - n]
-
-instance instGetElem : GetElem (ArrayMin n α) Nat α (fun arr i => i < arr.size) where
-  getElem self i h_i := self.get ⟨i, h_i⟩
-
-def get? (self : ArrayMin n α) (i : Nat) : Option α :=
-  if h : i < self.size
-  then self.get ⟨i, h⟩
-  else none
-
-def get! [Inhabited α] (self : ArrayMin n α) (i : Nat) : α :=
-  if let some a := self.get? i
-  then a
-  else panic! s!"illegal index {i} for `ArrayMin {n} _` of size {self.size}"
-
-def getN (i : Nat) (h : i < n := by decide) : α :=
-  have := self.pref_size ▸ h
-  self.pref[i]
-
-def toArray : Array α := self.pref ++ self.suff
-
-def toList : List α := self.pref.toList ++ self.suff.toList
-
-def push (a : α) : ArrayMin n α :=
-  {self with suff := self.suff.push a }
-
-def drainFirst : ArrayMin n.succ α → α × ArrayMin n α
-| ⟨⟨fst::pref⟩, h_pref', suff⟩ =>
-  (fst, ⟨
-    ⟨pref⟩,
-    by
-      simp at h_pref'
-      assumption,
-    suff
-  ⟩)
-
-instance instForIn : ForIn m (ArrayMin n α) α where
-  forIn self init f := do
-    let mut acc := init
-    for a in self.pref do
-      match ← f a acc with
-      | .done a => return a
-      | .yield a => acc := a
-    for a in self.suff do
-      match ← f a acc with
-      | .done a => return a
-      | .yield a => acc := a
-    return acc
-
-structure Frame (n : Nat) (α : Type u) : Type u where
-private mk ::
-  private pref : Array α := #[]
-  private suff : Array α := #[]
-deriving Inhabited
-
-namespace Frame
-def new (n : Nat) : Frame n α :=
-  ⟨#[], #[]⟩
-
-variable (self : Frame n α)
-
-def push (a : α) : Frame n α :=
-  if self.pref.size < n then
-    {self with pref := self.pref.push a}
-  else
-    {self with suff := self.suff.push a}
-
-def finalize [Inhabited α] : ArrayMin n α :=
-  if h : self.pref.size = n then
-    ⟨self.pref, h, self.suff⟩
-  else
-    panic! s!"[ArrayMin.finalize] unexpected prefix of size {self.pref.size}, expected {n}"
-end Frame
-
-def newFrame : ArrayMin n α → Frame n β
-| _ => Frame.new n
-
-structure Iter (n : Nat) (α : Type u) : Type u where
-private mk ::
-  val : ArrayMin n α
-  pos : Nat
-
-namespace Iter
-variable (self : Iter n α)
-
-abbrev isNotDone : Bool :=
-  self.pos < self.val.size
-abbrev isDone : Bool :=
-  ¬ self.isNotDone
-
-def next? : Option α × Iter n α :=
-  if h : self.isNotDone then
-    let next := self.val.get ⟨
-      self.pos,
-      by simp [isNotDone] at h ; simp [h]
-    ⟩
-    (next, {self with pos := self.pos.succ})
-  else (none, self)
-end Iter
-
-def iter : Iter n α :=
-  ⟨self, 0⟩
-
-end ArrayMin
+-- end Term.Kind
