Cvc/Basic/Env.lean
@@ -1,0 +1,219 @@
+/-
+Copyright (c) 2025 by the authors listed in the file AUTHORS and their
+institutional affiliations. All rights reserved.
+Released under Apache 2.0 license as described in the file LICENSE.
+Authors: Adrien Champion
+-/
+
+module
+
+import all Cvc.Basic.Error
+public import Cvc.Basic.Error
+public import cvc5
+
+
+
+/-! # `Ω` class and environment monad
+
+## `Ω` class
+
+Most of the types and functions in this library have an implicit `Ω`-class parameter. Under the hood
+cvc5 has a notion of *term manager*, and term/sort/solver/*etc.* can only be used with
+term/sort/solver/*etc.* if they user/are managed by the same term manager. Values of class `Ω`
+encode belonging to a specific term manager, causing compilation errors when two quantities are not
+guaranteed to agree on their manager.
+
+> Note that this library does not expose term managers directly, precisely to avoid runtime errors
+> related to using different term managers.
+
+`Ω`'s design is heavily inspired by `ST.Ref` and `StateRefT'`, and it provides the same *scoping*
+property: it is not possible to use an `Ω`-sort/term/solver/*etc.* after its underlying manager has
+been destroyed (which would cause a runtime error); see `Env.run` for details.
+
+## Environment monad
+
+Almost all sort/term/solver operations happen in the `Env` monad (and/or its transformer, `EnvT`).
+An `Ω`-`Env` allows creating and operating on `Ω`-sorts, `Ω`-terms, `Ω`-solvers, *etc.* which are
+guaranteed to be compatible.
+
+-/
+namespace Cvc public section
+
+open cvc5 renaming Error → Error5, TermManager → Tm, Env → Env5, EnvT → Env5T
+
+
+
+namespace Error
+/-- Conversion to `cvc5` errors. -/
+private def toUnsafe : Error → cvc5.Error
+| .internal "a value is missing" => .missingValue
+| .internal msg => .error s!"[internal] {msg}"
+| .unsupported msg => .unsupported msg
+| .user msg => .error msg
+| .io msg => .error s!"[io] {msg}"
+
+/-- Constructor from `cvc5` errors. -/
+private def ofUnsafe : cvc5.Error → Error
+| .missingValue => .internal "a value is missing"
+| .error msg => .internal s!"{msg}"
+| .option msg => .internal s!"option error: {msg}"
+| .unsupported msg => .unsupported msg
+| .recoverable msg => .internal s!"recoverable: {msg}"
+
+private instance : MonadLift (Except cvc5.Error) (Except Error) where
+  monadLift
+  | .ok res => .ok res
+  | .error e => .error (ofUnsafe e)
+end Error
+
+private def liftRes5 (code : Except Error5 α) : Except Error α := code.mapError Error.ofUnsafe
+
+
+
+class Ω : Prop where private mk ::
+
+structure EnvT [Ω] (m : Type → Type) (α : Type) : Type where private mk ::
+  private runOn : StateRefT' IO.RealWorld Tm (ResT m) α
+
+@[expose]
+def Env [Ω] : (α : Type) → Type := EnvT BaseIO
+
+namespace EnvT variable [Ω] [M : Monad m]
+
+protected def pure (a : α) : EnvT m α := ⟨fun _ => M.pure (.ok a)⟩
+
+protected def bind (code : EnvT m α) (f : α → EnvT m β) : EnvT m β where
+  runOn state := do
+    let a ← code.runOn state
+    f a |>.runOn state
+
+instance : Monad (EnvT m) where
+  pure := EnvT.pure
+  bind := EnvT.bind
+
+def liftBaseIO [MonadLiftT BaseIO m] (code : BaseIO α) : EnvT m α where runOn _ := code
+
+instance [MonadLiftT BaseIO m] : MonadLift BaseIO (EnvT m) := ⟨liftBaseIO⟩
+
+def liftIO [MonadLiftT BaseIO m] (code : IO α) : EnvT m α where runOn _ := do
+  match ← code.toBaseIO with
+  | .ok a => return a
+  | .error e => throwIO e
+
+instance [MonadLiftT BaseIO m] : MonadLift IO (EnvT m) := ⟨liftIO⟩
+
+def liftEnv [L : MonadLiftT BaseIO m] (code : Env α) : EnvT m α where
+  runOn := L.monadLift ∘ code.runOn
+
+instance [MonadLiftT BaseIO m] : MonadLift Env (EnvT m) := ⟨liftEnv⟩
+
+def liftResT (a? : ResT m α) : EnvT m α where
+  runOn _state := a?
+
+instance : MonadLift (ResT m) (EnvT m) := ⟨liftResT⟩
+example [L : MonadLiftT BaseIO m] : MonadLift Env (EnvT m) where
+  monadLift code := ⟨L.monadLift ∘ code.runOn⟩
+
+
+
+section sanity
+example : MonadLiftT Res (EnvT m) := inferInstance
+end sanity
+
+protected def throw (e : Error) : EnvT m α where
+  runOn _state := throw e
+
+protected def tryCatch (code : EnvT m α) (errorDo : Error → EnvT m α) : EnvT m α where
+  runOn state := try code.runOn state catch e => errorDo e |>.runOn state
+
+instance : MonadExceptOf Error (EnvT m) where
+  throw := EnvT.throw
+  tryCatch := EnvT.tryCatch
+
+instance : Inhabited (EnvT m α) where
+  default := throwInternal "`Inhabited` witness"
+
+instance : Inhabited (Env α) := inferInstanceAs (Inhabited (EnvT BaseIO α))
+
+private def liftRes5T : Except Error5 α → EnvT m α
+  | .ok a => ⟨fun _ => return a⟩
+  | .error e => ⟨fun _ => Error.ofUnsafe e |> throw⟩
+
+private def lift5 [MonadLiftT BaseIO m] (code : Env5T m α) : EnvT m α where
+  runOn state := do liftRes5T (← code.run) |>.runOn state
+
+end EnvT
+
+namespace Env variable [Ω]
+
+def liftBaseIO (code : BaseIO α) : Env α := EnvT.liftBaseIO code
+
+instance : MonadLift BaseIO Env := ⟨liftBaseIO⟩
+
+def liftIO (code : IO α) : Env α := EnvT.liftIO code
+
+instance : MonadLift IO Env := ⟨liftIO⟩
+
+export EnvT (lift5)
+
+instance : Monad Env := EnvT.instMonad
+
+instance : MonadLift (ResT BaseIO) Env := EnvT.instMonadLiftResT
+instance : MonadExceptOf Error Env := EnvT.instMonadExceptOfError
+
+instance : MonadLift (EnvT BaseIO) Env := ⟨id⟩
+
+-- private instance : MonadLift Env5 Env := EnvT.instMonadLiftEnvTOfMonadLiftTBaseIO
+
+section sanity
+example : MonadLiftT Res Env := inferInstance
+-- private example : MonadLiftT (Except Error5) Env := inferInstance
+end sanity
+
+end Env
+
+
+
+namespace EnvT
+
+def run [Monad m] [MonadLiftT BaseIO m] (code : [Ω] → EnvT m α) : m (Res α) := do
+  let _scope := Ω.mk
+  match ← Tm.new.run with
+  | .ok tm => IO.mkRef tm >>= code.runOn
+  | .error e => return Error.ofUnsafe e |> .error
+
+end EnvT
+
+namespace Env
+
+def run (code : [Ω] → Env α) : BaseIO (Res α) := EnvT.run code
+
+def runIO (code : [Ω] → Env α) : IO α := do
+  match ← run code with
+  | .ok a => return a
+  | .error e => IO.Error.userError e.toString |> throw
+
+end Env
+
+
+
+section variable [Ω]
+
+private def getManager : Env Tm := ⟨fun tmRef => tmRef.get⟩
+
+-- private def runUnsafe [Monad m'] [MonadLiftT BaseIO m] [Monad m] [MonadLiftT m' (EnvT m)]
+--   (code : cvc5.TermManager → m' α)
+-- : EnvT m α := do
+--   code (← getManager)
+
+-- private def runUnsafe' [Monad m'] [MonadLiftT BaseIO m] [Monad m] [MonadLiftT m' (EnvT m)]
+--   (code : m' α)
+-- : EnvT m α := runUnsafe fun _ => code
+
+
+private def runUnsafe [Monad m] [MonadLiftT BaseIO m]
+  (code : cvc5.TermManager → cvc5.EnvT m α)
+: EnvT m α := do EnvT.lift5 <| code (← getManager)
+
+private def runUnsafe' [Monad m] [MonadLiftT BaseIO m] (code : cvc5.EnvT m α) : EnvT m α :=
+  EnvT.lift5 code
