Cvc/Datatype.lean
@@ -1,0 +1,159 @@
+/-
+Copyright (c) 2026 by the authors listed in the file AUTHORS and their
+institutional affiliations. All rights reserved.
+Released under Apache 2.0 license as described in the file LICENSE.
+Authors: Adrien Champion
+-/
+
+module
+
+import all Cvc.Basic.Env
+import all Cvc.Untyped.Defs
+
+public import Cvc.Untyped.Defs
+
+
+
+namespace Cvc.Datatype variable [Ω]
+
+open cvc5 renaming Datatype → Dt, DatatypeDecl → DtD, DatatypeSelector → DtS
+open cvc5 renaming DatatypeConstructor → DtC, DatatypeConstructorDecl → DtCD
+
+
+
+namespace Constructor.Decl variable (d : Decl)
+
+@[inherit_doc DtCD.addSelector]
+def addSelector (name : String) (sort : Srt) : Env Decl :=
+  runUnsafe' do d.toUnsafe.addSelector name sort.toUnsafe
+
+@[inherit_doc DtCD.addSelectorSelf]
+def addSelectorSelf (name : String) : Env Decl :=
+  runUnsafe' do d.toUnsafe.addSelectorSelf name
+
+@[inherit_doc DtCD.addSelectorUnresolved]
+def addSelectorUnresolved (name : String) (unresDatatypeName : String) : Env Decl :=
+  runUnsafe' do d.toUnsafe.addSelectorUnresolved name unresDatatypeName
+
+end Constructor.Decl
+
+
+
+namespace Decl variable (d : Decl)
+
+@[inherit_doc DtD.addConstructor]
+def addConstructor (ctor : Constructor.Decl) : Env Decl :=
+  runUnsafe' do d.toUnsafe.addConstructor ctor.toUnsafe
+
+@[inherit_doc DtD.getNumConstructors]
+def countConstructors : Nat := d.toUnsafe.getNumConstructors
+
+@[inherit_doc DtD.isParametric]
+def isParametric : Bool := d.toUnsafe.isParametric
+
+@[inherit_doc DtD.getName]
+def getName : Res String := d.toUnsafe.getName
+
+@[inherit_doc DtD.isResolved]
+def isResolved : Env Bool := runUnsafe' do d.toUnsafe.isResolved
+
+end Decl
+
+
+
+namespace Selector variable (s : Selector)
+
+@[inherit_doc DtS.getName]
+def getName : Res String := s.toUnsafe.getName
+
+@[inherit_doc DtS.getTerm]
+def getTerm : Env Term := runUnsafe' do s.toUnsafe.getTerm
+
+@[inherit_doc DtS.getUpdaterTerm]
+def getUpdaterTerm : Env Term := runUnsafe' do s.toUnsafe.getUpdaterTerm
+
+@[inherit_doc DtS.getCodomainSort]
+def getCodomainSort : Env Srt := runUnsafe' do s.toUnsafe.getCodomainSort
+
+end Selector
+
+
+
+namespace Constructor variable (c : Constructor)
+
+@[inherit_doc DtC.getName]
+def getName : Res String := c.toUnsafe.getName
+
+def getTerm : Env Term := runUnsafe' do c.toUnsafe.getTerm
+
+def getInstantiatedTerm (retSort : Srt) : Env Term :=
+  runUnsafe' do c.toUnsafe.getInstantiatedTerm retSort
+
+def getTesterTerm : Env Term :=
+  runUnsafe' do c.toUnsafe.getTesterTerm
+
+def countSelectors : Nat := c.getNumSelectors
+
+@[inherit_doc DtC.getSelector]
+def getSelector (name : String) : Env Selector :=
+  runUnsafe' do c.toUnsafe.getSelector name
+
+@[inherit_doc DtC.getSelectorAt]
+def getSelectorAt (idx : Fin c.countSelectors) : Selector := c.toUnsafe.getSelectorAt idx
+
+instance : GetElem Constructor Nat Selector fun c idx => idx < c.countSelectors :=
+  inferInstanceAs (GetElem DtC Nat DtS fun c idx => idx < c.getNumSelectors)
+
+instance [Monad m] : ForIn m Constructor Selector := inferInstanceAs (ForIn m DtC DtS)
+
+end Constructor
+
+
+
+section variable (dt : Datatype)
+
+@[inherit_doc Dt.getConstructor]
+def getConstructor (name : String) : Env Constructor :=
+  runUnsafe' do dt.toUnsafe.getConstructor name
+
+@[inherit_doc Dt.getNumConstructors]
+def countConstructors : Nat := dt.toUnsafe.getNumConstructors
+
+@[inherit_doc Dt.getConstructorAt]
+def getConstructorAt (idx : Fin dt.countConstructors) : Constructor :=
+  dt.toUnsafe.getConstructorAt idx
+
+instance : GetElem Datatype Nat Constructor fun dt idx => idx < dt.countConstructors :=
+  inferInstanceAs (GetElem Dt Nat DtC fun dt idx => idx < dt.getNumConstructors)
+
+instance [Monad m] : ForIn m Datatype Constructor := inferInstanceAs (ForIn m Dt DtC)
+
+@[inherit_doc Dt.getSelector]
+def getSelector (name : String) : Env Selector :=
+  runUnsafe' do dt.toUnsafe.getSelector name
+
+@[inherit_doc Dt.getName]
+def getName : Res String := dt.toUnsafe.getName
+
+@[inherit_doc Dt.getParameters]
+def getParameters : Env (Array Srt) := runUnsafe' do dt.toUnsafe.getParameters
+
+@[inherit_doc Dt.isParametric]
+def isParametric : Bool := dt.toUnsafe.isParametric
+
+@[inherit_doc Dt.isCodatatype]
+def isCoDatatype : Bool := dt.toUnsafe.isCodatatype
+
+@[inherit_doc Dt.isTuple]
+def isTuple : Bool := dt.toUnsafe.isTuple
+
+@[inherit_doc Dt.isRecord]
+def isRecord : Bool := dt.toUnsafe.isRecord
+
+@[inherit_doc Dt.isFinite]
+def isFinite : Res Bool := dt.toUnsafe.isFinite
+
+@[inherit_doc Dt.isWellFounded]
+def isWellFounded : Bool := dt.toUnsafe.isWellFounded
+
+end
