Cvc/Extra/Actlit.lean
@@ -1,0 +1,77 @@
+/-
+Copyright (c) 2026 by the authors listed in the file AUTHORS and their
+institutional affiliations. All rights reserved.
+Released under Apache 2.0 license as described in the file LICENSE.
+Authors: Adrien Champion
+-/
+
+module
+
+-- public import Cvc.Basic.Batteries
+public import Cvc.Solver
+
+
+
+namespace Cvc variable [Ω]
+
+def Actlit := Term
+
+namespace Actlit
+
+section variable (a1 a2 : Actlit)
+
+protected def beq : Bool := Term.beq a1 a2
+protected def compare : Ordering := Term.compare a1 a2
+
+instance : BEq Actlit := ⟨Actlit.beq⟩
+instance : Ord Actlit := ⟨Actlit.compare⟩
+
+end
+
+structure Core where
+private mk ::
+  private nextIdx : Nat
+  -- private live : RBSet Actlit
+
+protected abbrev EnvT (m : Type → Type) : (α : Type) → Type :=
+  StateRefT' IO.RealWorld Core (EnvT m)
+
+protected abbrev Env : (α : Type) → Type := Actlit.EnvT BaseIO
+
+namespace EnvT
+
+instance [MonadLiftT BaseIO m] : MonadLift (Cvc.EnvT m) (Actlit.EnvT m) where
+  monadLift code := fun _ => code
+
+end EnvT
+
+private def mkNameOfNat (idx : Nat) : String :=
+  s!"__cvc__actlit__{idx}"
+
+def mk : Actlit.Env Actlit := do
+  let core ← getThe Core
+  let name := mkNameOfNat core.nextIdx
+  let actlit ← Term.mkConst name (← Srt.bool)
+  -- if core.live.contains actlit then
+  --   throwInternal s!"fresh actlit {actlit} already registered in the set of live actlits"
+  set {core with nextIdx := core.nextIdx.succ,
+    -- live := core.live.insert actlit
+  }
+  return actlit
+
+section variable (a : Actlit)
+
+protected def toString : String := Term.toString a
+instance : ToString Actlit := ⟨Actlit.toString⟩
+
+def activateIn (solver : Solver) (term : Term) : Cvc.Env Unit :=
+  a.implies term >>= solver.assert
+
+def deactivateIn (solver : Solver) : Cvc.Env Unit := do
+  -- let core ← getThe Core
+  -- set {core with live := core.live.erase a}
+  solver.assert (← a.not)
+
+end
+
+end Actlit
