Cvc/Extra/StateVars.lean
@@ -1,0 +1,36 @@
+/-
+Copyright (c) 2026 by the authors listed in the file AUTHORS and their
+institutional affiliations. All rights reserved.
+Released under Apache 2.0 license as described in the file LICENSE.
+Authors: Adrien Champion
+-/
+
+module
+
+public import Cvc.Solver
+
+
+
+namespace Cvc
+
+
+
+abbrev StateVars.Sig := (Var : Type) → Type
+
+class StateVars (S : StateVars.Sig) where
+  init [Monad m] [Ω] : (s : S String) → (f : String → Srt → m α) → m (S α)
+  foldM [Monad m] : (s : S α) → (f : β → α → m β) → (init : β) → m (S β)
+  mapM [Monad m] : (s : S α) → (f : α → m β) → m (S β)
+
+section variable [Ω] [SVars : StateVars S]
+
+def declareStateVars (s : S String) : Env (S Term) := SVars.init s Term.mkConst
+
+def Solver.getStateVarValues (solver : Solver) (s : S Term) : EnvSat (S Term) :=
+  SVars.mapM s solver.getValue
+
+end
+
+
+-- syntax atomic((declModifiers true) "state_vars ") $id:ident (" where " <|> " := ") ppLineIndent
+--   ( (declModifiers true) rawIdent )*
