Cvc/Patterns.lean
@@ -1,0 +1,256 @@
+/-
+Copyright (c) 2026 by the authors listed in the file AUTHORS and their
+institutional affiliations. All rights reserved.
+Released under Apache 2.0 license as described in the file LICENSE.
+Authors: Adrien Champion
+-/
+
+module
+
+public meta import Lean.Elab.Command
+public import Cvc.Basic.Env
+
+import all Cvc.Srt
+import all Cvc.Term
+
+public import Cvc.Term
+
+
+
+namespace Cvc public section variable [Ω]
+
+
+syntax (name := patTreeStx)
+  atomic(declModifiers ppLine "pat_tree")
+  "[" ident ident ", " ident ", " term "]"
+  ident ", " ident (
+    group(
+      (docComment)?
+      ppLine "| " declModifiers rawIdent "[" term "]"
+        ( "(" rawIdent " : " term " ← " doSeq ")" )*
+        ppLine ppIndent("→ " doSeq)
+    )
+  )* : command
+
+section
+open Lean Elab Command
+
+
+syntax "𝓢ub" : term
+syntax "𝓡es" : term
+
+@[command_elab patTreeStx]
+public meta def elabPatTreeStx : CommandElab
+| `(
+  $mods:declModifiers
+  pat_tree[$ofActual:ident $ofActualInput:ident, $toActual:ident, $actualTy:term]
+  $patternId:ident, $treeId:ident $[
+    $[ $variantDoc?:docComment ]?
+    | $variantMods:declModifiers $variantId:ident [ $actualVariantId:term ]
+      $[ ( $variantArgs:ident : $variantArgsTy:term ← $variantArgsOfActual:doSeq ) ]*
+      → $variantToActual:doSeq
+  ]*
+) => do
+  let toStringId := mkIdent `toString
+  let envId := mkIdent ``Env
+  let patId := mkIdent `Pat
+  let patTyParam := mkIdent `α
+  let patTy ← `( $patId $patTyParam )
+  let binderss ← variantArgs.zip variantArgsTy |>.mapM fun (args, tys) => do
+    let binders : Array _ ← args.zip tys |>.mapM fun (args, ty) => do
+      let raw ← ty.raw |> Lean.Syntax.replaceM fun
+        | `(𝓢ub) => return some patTyParam.raw
+        | `(𝓡es) => return some patTy.raw
+        | _ => return none
+      let ty := {ty with raw}
+      `(bracketedBinder| ( $args:ident : $ty ) )
+    return binders
+  let stx ← `(
+    $mods:declModifiers
+    inductive $patId:ident ($patTyParam : Type) $[
+      $[ $variantDoc?:docComment ]?
+      | $variantMods:declModifiers $variantId:ident $[ $binderss:bracketedBinder ]*
+    ]*
+    deriving Inhabited, BEq, Ord, Hashable, Repr
+
+    namespace $patId
+    instance [Repr $patTyParam] : ToString ($patId $patTyParam) := ⟨(s!"{reprPrec · 0}")⟩
+
+    /-- String representation. -/
+    protected def $toStringId [Repr $patTyParam] : $patId $patTyParam → String := $toStringId
+    end $patId
+  )
+  -- logInfo s!"elaborating consultation:\n{← liftCoreM <| Lean.PrettyPrinter.formatTerm stx}"
+  elabCommand stx
+
+  let stx ← `(
+    $mods:declModifiers
+    abbrev $patternId := $patId $actualTy
+  )
+  elabCommand stx
+
+  let treeIntroId := mkIdent `intro
+  let patToStringId := patId.getId.append toStringId.getId |> mkIdent
+  let treeToStringId := treeId.getId.append toStringId.getId |> mkIdent
+  let stx ← `(
+    $mods:declModifiers
+    inductive $treeId
+    | $treeIntroId:ident : $patId $treeId → $treeId
+    deriving Inhabited, BEq, Ord, Hashable, Repr
+
+    namespace $treeId
+    /-- String representation. -/
+    protected def $toStringId : $treeId → String
+      | .$treeIntroId pat => $patToStringId pat
+    instance : ToString $treeId := ⟨$treeToStringId⟩
+    end $treeId
+  )
+  elabCommand stx
+
+  let variants :=
+    variantDoc?.zip <| variantId.zip <| variantArgs
+  for (variantDoc?, variantId, args) in variants do
+    let patternVariantId := patId.getId.append variantId.getId |> mkIdent
+    let stx ← `(
+      namespace $treeId
+      $[ $variantDoc?:docComment ]?
+      @[match_pattern]
+      abbrev $variantId:ident $[$args:ident]* :=
+        ( $treeIntroId <| $patternVariantId:ident $[ $args:ident ]* )
+      end $treeId
+    )
+    elabCommand stx
+
+  let patToActualId := patId.getId.append toActual.getId |> mkIdent
+  let ofPatternId := mkIdent `ofPattern
+  let ofTreeId := mkIdent `ofTree
+  let patternToActualId := patternId.getId.append toActual.getId |> mkIdent
+  let treeToActualId := treeId.getId.append toActual.getId |> mkIdent
+  let stx ← `(
+    namespace $patId
+    def $toActual ($toActual : $patTyParam → $envId $actualTy)
+    : $patId $patTyParam → $envId $actualTy
+      $[ | $variantId:ident $[ $variantArgs:ident]* => do $variantToActual:doSeq ]*
+    end $patId
+
+    namespace $patternId
+    def $toActual : (pat : $patternId) → $envId $actualTy := $patToActualId pure
+    end $patternId
+
+    def $ofPatternId := $patternToActualId
+
+    namespace $treeId
+    partial def $toActual : (tree : $treeId) → $envId $actualTy
+      | $treeIntroId pat => $patToActualId $toActual pat
+    end $treeId
+
+    def $ofTreeId := $treeToActualId
+  )
+  elabCommand stx
+
+  let patOfActualId := patId.getId.append ofActual.getId |> mkIdent
+  let toPatternId := mkIdent `toPattern
+  let toTreeId := mkIdent `toTree
+  let patternOfActualId := patternId.getId.append ofActual.getId |> mkIdent
+  let treeOfActualId := treeId.getId.append ofActual.getId |> mkIdent
+  let variantArgs' := variantArgs
+  let stx ← `(
+    namespace $patId
+    def $ofActual
+      ($ofActual : $actualTy → $envId $patTyParam) ($ofActualInput : $actualTy)
+    : $envId ($patId $patTyParam) := do
+      match ← ($ofActualInput |>.getKind) with
+      $[ | $actualVariantId =>
+        $[ let $variantArgs ← do $variantArgsOfActual ]*
+        return $variantId $[ $variantArgs' ]*
+      ]*
+      | k => throwInternal s!"unsupported kind {k}"
+    end $patId
+
+    namespace $patternId
+    def $ofActual : ($ofActualInput : $actualTy) → $envId $patternId := $patOfActualId pure
+    end $patternId
+
+    def $toPatternId := $patternOfActualId
+
+    namespace $treeId
+    partial def $ofActual ($ofActualInput : $actualTy) : $envId $treeId :=
+      $treeIntroId <$> $patOfActualId $ofActual $ofActualInput
+    end $treeId
+
+    def $toTreeId := $treeOfActualId
+  )
+  elabCommand stx
+
+| _ => throwUnsupportedSyntax
+
+end
+
+
+
+namespace Srt
+
+/-- A pattern-matchable version of `Srt`. -/
+pat_tree[ofSrt srt, toSrt, Srt] Pattern, Tree
+
+| bool [.BOOLEAN_SORT] → Srt.bool
+| int [.INTEGER_SORT] → Srt.int
+| real [.REAL_SORT] → Srt.real
+| regex [.REGLAN_SORT] → Srt.regex
+| roundingMode [.ROUNDINGMODE_SORT] → Srt.roundingMode
+| string [.STRING_SORT] → Srt.string
+
+| abstract [.ABSTRACT_SORT]
+  (a : Abstract ← Abstract.ofKind (← srt.getAbstractedKind))
+→ a.toSrt
+
+| bag [.BAG_SORT]
+  (elm : 𝓢ub ← srt.getBagElementSort >>= ofSrt)
+→ toSrt elm >>= Srt.bag
+
+| array [.ARRAY_SORT]
+  (idx : 𝓢ub ← srt.getArrayIndexSort >>= ofSrt)
+  (elm : 𝓢ub ← srt.getArrayElementSort >>= ofSrt)
+→ (← toSrt idx).arrayTo (← toSrt elm)
+
+| bitVec [.BITVECTOR_SORT]
+  (size : UInt32 ← srt.getBitVectorSize)
+→ Srt.bitVec size
+
+| float [.FLOATINGPOINT_SORT]
+  (exp : UInt32 ← srt.getFloatingPointExponentSize)
+  (sig : UInt32 ← srt.getFloatingPointSignificandSize)
+→ Srt.float exp sig
+
+| finiteField [.FINITE_FIELD_SORT]
+  (size : Nat ← srt.getFiniteFieldSize)
+→ Srt.finiteField size
+
+| function [.FUNCTION_SORT]
+  (dom : Array 𝓢ub ← srt.getFunctionDomainSorts >>= Array.mapM ofSrt)
+  (cod : 𝓢ub ← srt.getFunctionCodomainSort >>= ofSrt)
+→ let dom ← dom.mapM toSrt
+  if h : 0 < dom.size then toSrt cod >>= Srt.function dom
+  else throwInternal "ill-formed pattern: function with empty domain"
+
+end Srt
+
+
+
+namespace Term
+
+/-- A pattern-matchable version of `Term`. -/
+pat_tree[ofTerm term, toTerm, Term] Pattern, Tree
+| bool [.CONST_BOOLEAN]
+  (b : Bool ← term.getBoolValue)
+→ Term.mkBool b
+
+| int [.CONST_INTEGER]
+  (i : Int ← term.getIntValue)
+→ Term.mkInt i
+
+| string [.CONST_STRING]
+  (s : String ← term.getStringValue)
+→ Term.mkString s
+
+end Term
