Cvc/Tests/Untyped/TestArray.lean
@@ -1,0 +1,45 @@
+module
+
+import Cvc.Untyped.Types.Array
+
+import Cvc.Tests.TestBasic
+
+
+
+namespace Cvc.Untyped.Tests
+
+/-- info:
+((as const (Array Bool Int)) 7)
+→ { _ ↦ 7 }
+(store ((as const (Array Bool Int)) 7) true 13)
+→ { true ↦ 13, _ ↦ 7 }
+(store (store ((as const (Array Bool Int)) 7) true 13) false 5)
+→ { true ↦ 13, false ↦ 5, _ ↦ 7 }
+(store (store (store ((as const (Array Bool Int)) 7) true 13) false 5) true 7)
+→ { true ↦ 7, false ↦ 5, _ ↦ 7 }
+→ { false ↦ 5, true ↦ 7, _ ↦ 7 }
+-/
+#test basic.array.creation do
+  let int ← Srt.int
+  let bool ← Srt.bool
+  let five ← Term.mkInt 5
+  let seven ← Term.mkInt 7
+  let thirteen ← Term.mkInt 13
+  let tru ← Term.mkValue true
+  let fls ← Term.mkValue false
+  let arraySrt ← bool.arrayTo int
+  let array ← Term.mkArray arraySrt (default := seven)
+  println! "{array}"
+  println! "→ {← array.getArrayValue}"
+  let array ← array.store tru thirteen
+  println! "{array}"
+  println! "→ {← array.getArrayValue}"
+  let array ← array.store fls five
+  println! "{array}"
+  println! "→ {← array.getArrayValue}"
+  let array ← array.store tru seven
+  println! "{array}"
+  let arrayValue ← array.getArrayValue
+  println! "→ {arrayValue}"
+  let tMap ← arrayValue.termsToValues Bool Int
+  println! "→ {tMap}"
