Cvc/Tests/Untyped/TestSolver.lean
@@ -1,0 +1,43 @@
+module
+
+import Cvc.Untyped.Term
+import Cvc.Untyped.Solver
+
+import Cvc.Tests.TestBasic
+
+
+
+namespace Cvc.Untyped.Tests
+
+
+
+/--
+info: s1 : (Seq Int) := s1
+→ (seq.++ (seq.unit 0) (seq.unit 1) (seq.unit 2))
+→ #[0, 1, 2]
+-/
+#test array.getValue do
+  let solver ← Solver.new
+  solver.setOption "produce-models" "true"
+  -- let bool ← Srt.bool
+  let int ← Srt.int
+  let seqBool ← int.seq
+  let s1 ← Term.mkSymbol "s1" seqBool
+  println! "s1 : {← s1.getSort} := {s1}"
+  let i0 ← Term.mkValue 0
+  let i1 ← Term.mkValue 1
+  let i2 ← Term.mkValue 2
+  -- let tru ← Term.mkValue true
+  -- let fls ← Term.mkValue false
+  let atEq (idx val : Term) : Env Term := do
+    let tAt ← s1.seqAt idx
+    val.unitSeq >>= tAt.equal
+  atEq i0 i0 >>= solver.assert
+  atEq i1 i1 >>= solver.assert
+  atEq i2 i2 >>= solver.assert
+  let val ← solver.checkSat (ifSat := do
+    let value ← solver.getValue s1
+    return value)
+  println! "→ {val}"
+  let v ← val.getSeqValue (α := Int)
+  println! "→ {v}"
