Cvc/Tests/Untyped/TestSrt.lean
@@ -1,0 +1,79 @@
+module
+
+import Cvc.Untyped.Srt
+
+import Cvc.Tests.TestBasic
+
+namespace Cvc.Tests
+
+
+
+/- Making sure the API works as we expect -/
+
+set_option linter.unusedVariables false in
+/--
+info: - Bool
+- Int
+- (-> Int Bool)
+- (Array Bool (-> Int Bool))
+- (-> Bool (Array Bool (-> Int Bool)))
+- (Bag (-> Bool (Array Bool (-> Int Bool))))
+- (Bag (-> Int Bool))
+- (Set (-> Bool (Array Bool (-> Int Bool))))
+- (Set (-> Int Bool))
+- (Seq (-> Bool (Array Bool (-> Int Bool))))
+- (Seq (-> Int Bool))
+Error:
+- [internal] invalid argument '(-> Int Bool)' for 'codomain', expected non-function sort as codomain sort
+-/
+#test basic.sort.creation do
+  let printMk (code : Env Srt) : Env Srt := do
+    let srt ← code
+    println! "- {srt}"
+    return srt
+  let printError {α : Type} (desc : String) (code : Env α) : Env Unit := do
+    try
+      let _ ← code
+      throwUser s!"{desc}: expected an error, got success"
+    catch e => println! "Error:\n- {e}"
+  let bool ← printMk Srt.bool
+  let int ← printMk Srt.int
+  let fn ← printMk do Srt.function #[int] bool
+  let arrayFn ← printMk do bool.arrayTo fn
+  let fn2 ← printMk do Srt.function #[bool] arrayFn
+  let bag ← printMk do fn2.bag
+  let bag' ← printMk do fn.bag
+  let set ← printMk do fn2.set
+  let set' ← printMk do fn.set
+  let seq ← printMk do fn2.seq
+  let seq' ← printMk do fn.seq
+  printError "function with function codomain" do fn.function #[int]
+
+
+
+#test array.sort.creation do
+  let int ← Srt.int
+  let real ← Srt.real
+  let intToReal ← int.arrayTo real
+  intToReal |> assertString "(Array Int Real)"
+  real.array >>= assertEq intToReal
+  int.arrayFrom real >>= assertString "(Array Real Int)"
+
+#test function.sort.creation do
+  let bool ← Srt.bool
+  let int ← Srt.int
+  let real ← Srt.real
+  Srt.function #[int] real >>= assertString "(-> Int Real)"
+  Srt.function #[bool, int] real >>= assertString "(-> Bool Int Real)"
+
+/--
+error: could not synthesize default value for parameter 'domNonempty' using tactics
+---
+error: failed to prove the domain is nonempty
+inst✝ : Ω
+real : Srt
+⊢ 0 < #[].size
+-/
+#test! function.creation.error do
+  let real ← Srt.real
+  Srt.function #[] real >>= assertString "(-> Int Real)"
