Cvc/Tests/Untyped/TestSymbols.lean
@@ -1,0 +1,87 @@
+module
+
+import Cvc.Untyped.Symbols
+import Cvc.Ext
+
+import Cvc.Tests.TestBasic
+
+
+
+namespace Cvc.Untyped.Tests variable [Ω]
+
+open Cvc.Tests
+
+structure MySymbols (Sym : Type → Type) where
+  b1 : Sym Bool
+  b2 : Sym Bool
+  i1 : Sym Int
+  str1 : Sym String
+  seq1 : Sym (Array String)
+
+namespace MySymbols
+
+instance : Symbols MySymbols where
+  foldM
+  | {b1, b2, i1, str1, seq1}, f, init =>
+    f init b1 >>= (f · b2) >>= (f · i1) >>= (f · str1) >>= (f · seq1)
+  mapM
+  | {b1, b2, i1, str1, seq1}, f =>
+    return { b1 := ← f b1, b2 := ← f b2, i1 := ← f i1, str1 := ← f str1, seq1 := ← f seq1 }
+
+abbrev Idents := Symbols.Idents MySymbols
+abbrev Terms := Symbols.Terms MySymbols
+abbrev Values := Symbols.Values MySymbols
+
+def idents : MySymbols.Idents where
+  b1 := Symbol.mk "b1"
+  b2 := Symbol.mk "b2"
+  i1 := Symbol.mk "i1"
+  str1 := Symbol.mk "str1"
+  seq1 := Symbol.mk "seq1"
+
+end MySymbols
+
+def idents := MySymbols.idents
+
+/-- info:
+values:
+  b1 ↦ true
+  b2 ↦ true
+  i1 ↦ 1
+  str1 ↦ neko
+  seq1 ↦ #[, , , ]
+-/
+#test symbols.declareAndValues do
+  let vars ← idents.declare
+  let solver ← Solver.new
+  solver.setOption "produce-models" "true"
+
+  smt! vars.b1 ∨ 0 < - vars.i1
+    >>= solver.assert
+
+  let myAssertion ← smt! vars.b1 ∨ 0 < - vars.i1
+  solver.assert myAssertion
+
+
+  let myAssertion' ← smt! 1 = if vars.b2 then vars.i1 else 5 * vars.i1
+  solver.assert myAssertion'
+
+  let str1 ← smt! "ne"
+  let str2 ← smt! "ko"
+  let strConcat ← str1.stringConcat str2
+  let constraint ← smt! vars.str1 = strConcat
+  solver.assert constraint
+
+  let seq1Len ← vars.seq1.get.seqLength
+  let str1Len ← vars.str1.get.stringLength
+  smt! seq1Len = str1Len >>= solver.assert
+
+  let some {b1, b2, i1, str1, seq1} ← solver.checkSat? (ifSat := some <$> vars.getValues solver)
+    | throwUser "expected sat result"
+
+  println! "values:"
+  println! "  b1 ↦ {b1.get}"
+  println! "  b2 ↦ {b2.get}"
+  println! "  i1 ↦ {i1.get}"
+  println! "  str1 ↦ {str1.get}"
+  println! "  seq1 ↦ {seq1.get}"
