Cvc/Typed/Solver.lean
@@ -1,0 +1,126 @@
+module
+
+import all Cvc.Untyped.Solver
+import all Cvc.Typed.Term
+
+public import Cvc.Untyped.Solver
+public import Cvc.Typed.Term
+
+
+
+namespace Cvc.Typed public section variable [Ω]
+
+open Cvc.Untyped renaming Solver → S
+
+
+
+abbrev Solver := S
+
+export Cvc.Untyped (EnvSatT EnvSat EnvUnsatT EnvUnsat EnvUnknownT EnvUnknown)
+
+namespace Solver variable (s : Solver)
+
+export Cvc.Untyped.Solver (Result)
+open Cvc.Untyped.Solver (Result)
+
+def new : Env Solver := S.new
+
+def get : Solver → S := id
+
+def getAssertions : Env (Terms Bool) := S.getAssertions s
+
+def assert (t : Term Bool) : Env Unit := S.assert s t
+
+
+
+section check_sat variable [Monad m] [MonadLiftT BaseIO m] (assuming : Option (Terms Bool) := none)
+
+/-- Checks the satisfiability of the constraints asserted so far. -/
+def checkSatResult : Env Result := S.checkSatResult s (assuming := assuming)
+
+@[inherit_doc checkSatResult]
+def checkIsSat? : Env Result.Sat? := do
+  let res ← s.checkSatResult assuming
+  res.isSat?
+
+@[inherit_doc checkSatResult]
+def checkIsSat : Env Bool := do
+  let res ← s.checkSatResult assuming
+  res.isSat
+
+@[inherit_doc checkSatResult]
+def checkSat
+  (ifSat : EnvSatT m α := liftM (S.unexpectedSat s))
+  (ifUnsat : EnvUnsatT m α := s.unexpectedUnsat)
+  (ifUnknown : Unknown.Explanation → EnvUnknownT m α := liftM ∘ s.unexpectedUnknown)
+: EnvT m α := do
+  match ← s.checkIsSat? (assuming := assuming) with
+  | .inl true => ifSat.toEnv
+  | .inl false => ifUnsat.toEnv
+  | .inr unkExpl => ifUnknown unkExpl |>.toEnv
+
+@[inherit_doc checkSatResult]
+def checkSat?
+  (ifSat : EnvSatT m (Option α) := return none)
+  (ifUnsat : EnvUnsatT m (Option α) := return none)
+  (ifUnknown : Unknown.Explanation → EnvUnknownT m (Option α) := liftM ∘ s.unexpectedUnknown)
+: EnvT m (Option α) :=
+  s.checkSat assuming ifSat ifUnsat ifUnknown
+
+end check_sat
+
+
+
+section sat
+
+@[inherit_doc S.getValue]
+def getValueTerm (term : Term α) : EnvSat (Term α) := s.getValue term
+@[inherit_doc S.getValues]
+def getValueTerms (terms : Terms α) : EnvSat (Terms α) :=
+  runUnsafe' do s.toUnsafe.getValues terms
+
+@[inherit_doc getValueTerm]
+def getValue [TermToValue α] (s : Solver) (term : Term α) : EnvSat α := do
+  let valTerm ← s.getValueTerm term
+  valTerm.getValue
+@[inherit_doc getValueTerms]
+def getValues [TermToValue α] (s : Solver) (ts : Terms α) : EnvSat (Array α) := do
+  let valTerms ← s.getValueTerms ts
+  valTerms.mapM (Term.getValue ·)
+
+@[inherit_doc S.isModelCoreSymbol]
+def isModelCoreSymbol (term : Term α) : EnvSat Bool :=
+  runUnsafe' do s.toUnsafe.isModelCoreSymbol term
+
+end sat
+
+
+
+section unsat
+
+@[inherit_doc S.getUnsatAssumptions]
+def getUnsatAssumptions: EnvUnsat (Terms Bool) := runUnsafe' do s.toUnsafe.getUnsatAssumptions
+
+@[inherit_doc S.getUnsatCore]
+def getUnsatCore : EnvUnsat (Terms Bool) := runUnsafe' do s.toUnsafe.getUnsatCore
+
+@[inherit_doc S.getUnsatCoreLemmas]
+def getUnsatCoreLemmas : EnvUnsat (Terms Bool) := runUnsafe' do s.toUnsafe.getUnsatCoreLemmas
+
+end unsat
+
+
+
+section unknown
+
+@[inherit_doc S.getTimeoutCore]
+def getTimeoutCore : EnvUnknown (cvc5.Result × Terms Bool) :=
+  runUnsafe' do s.toUnsafe.getTimeoutCore
+
+@[inherit_doc S.getTimeoutCoreAssuming]
+def getTimeoutCoreAssuming (assumptions : Terms Bool) : EnvUnknown (cvc5.Result × Terms Bool) :=
+  runUnsafe' do s.toUnsafe.getTimeoutCoreAssuming assumptions
+
+end unknown
+
+end Solver
