Cvc/Typed/Symbols.lean
@@ -1,0 +1,96 @@
+/-
+Copyright (c) 2025 by the authors listed in the file AUTHORS and their
+institutional affiliations. All rights reserved.
+Released under Apache 2.0 license as described in the file LICENSE.
+Authors: Adrien Champion
+-/
+
+module
+
+import Cvc.Typed.Solver
+
+
+
+namespace Cvc.Typed variable [Ω] open Cvc.Typed renaming Term → T
+
+
+
+structure Symbol (F : Type → Type) (α : Type) where
+  get : F α
+
+
+namespace Symbol
+
+instance : Coe (Symbol F α) (F α) := ⟨get⟩
+
+abbrev Ident := Symbol (𝕂 String)
+
+abbrev Value := Symbol Id
+
+abbrev Term := Symbol T
+
+structure TermAt (k : Nat) (α : Type) extends toTerm : Term α where private mk' ::
+
+structure ValueAt (k : Nat) (α : Type) extends toValue : Value α where private mk' ::
+
+/-- The `Cvc.Typed.Term` in a `Symbol.Term`. -/
+def toTerm (symbol : Term α) : T α := symbol.get
+
+def declare [ToTyp α] (symbol : Ident α) : Env (Term α) :=
+  return { symbol with get := ← Term.mkSymbol symbol.get }
+
+def declareAt [ToTyp α] (symbol : Ident α) (k : Nat) : Env (TermAt k α) :=
+  let ident := s!"{symbol.get}__@__{k}"
+  return { get := ← Term.mkSymbol ident }
+
+def getValue [TermToValue α] (symbol : Term α) (solver : Solver) : EnvSat (Value α) :=
+  return {get := ← solver.getValue symbol.get}
+
+def getValueTerm (symbol : Term α) (solver : Solver) : EnvSat (Term α) :=
+  return {get := ← solver.getValueTerm symbol.get}
+
+namespace TermAt
+
+def mk [ToTyp α] (symbol : Ident α) (k : Nat) : Env (TermAt k α) :=
+  symbol.declareAt k
+
+def getValue [TermToValue α] (symbol : TermAt k α) (solver : Solver) : EnvSat (ValueAt k α) :=
+  return {get := ← solver.getValue symbol.get}
+
+def getValueTerm [TermToValue α] (symbol : TermAt k α) (solver : Solver) : EnvSat (TermAt k α) :=
+  return {get := ← solver.getValueTerm symbol.get}
+
+end TermAt
+
+end Symbol
+
+
+
+class Symbols (S : (Type → Type) → Type) where
+  mapM [Monad m] {F' : Type → Type} (syms : S F)
+    (f : {α : Type} → [ToTyp α] → [TermToValue α] → F α → m (F' α))
+  : m (S F')
+
+namespace Symbols
+
+abbrev Idents (S : (Type → Type) → Type) [Symbols S] := S Symbol.Ident
+abbrev Terms (S : (Type → Type) → Type) [Symbols S] := S Symbol.Term
+abbrev TermsAt (k : Nat) (S : (Type → Type) → Type) [Symbols S] := S (Symbol.TermAt k)
+abbrev Values (S : (Type → Type) → Type) [Symbols S] := S Symbol.Value
+abbrev ValuesAt (k : Nat) (S : (Type → Type) → Type) [Symbols S] := S (Symbol.ValueAt k)
+
+variable [inst : Symbols S]
+
+def declare (syms : Idents S) : Env (Terms S) :=
+  inst.mapM syms fun sym => sym.declare
+
+def declareAt (syms : Idents S) : Env (TermsAt k S) :=
+  inst.mapM syms fun sym => sym.declareAt k
+
+def Terms.getValues (syms : Terms S) (solver : Solver) : EnvSat (Values S) :=
+  inst.mapM syms fun sym => sym.getValue solver
+
+def TermsAt.getValues (syms : TermsAt k S) (solver : Solver) : EnvSat (ValuesAt k S) :=
+  inst.mapM syms fun sym => sym.getValue solver
+
+end Symbols
