Cvc/Typed/Term.lean
@@ -1,0 +1,300 @@
+module
+
+import all Cvc.Basic.Env
+import all Cvc.Untyped.Term
+import all Cvc.Typed.Defs
+
+public import Cvc.Typed.Defs
+public import Cvc.Untyped.Term
+
+
+
+namespace Cvc.Typed public section variable [Ω]
+
+open Cvc renaming Untyped.Term → T, Untyped.Terms → Ts
+
+
+
+macro
+  "def% " id:ident sig:optDeclSig " := " body:term
+: command => do
+  let fnId := ``T |>.append id.getId |> Lean.mkIdent
+  `(@[inherit_doc $fnId] def $id $sig := $body)
+
+macro
+  "def% " id:ident sig:optDeclSig " ← " expl?:("@")? fnId:ident
+: command => do
+  let fnId := ``T |>.append fnId.getId |> Lean.mkIdent
+  let fnTerm ← if expl?.isSome then `(@ $fnId _) else pure fnId
+  `(@[inherit_doc $fnId] def $id $sig := $fnTerm)
+macro
+  "def% " expl?:("@")? id:ident sig:optDeclSig
+: command => do
+  if expl?.isSome then `(def% $id:ident $sig:optDeclSig ← @ $id)
+  else `(def% $id:ident $sig:optDeclSig ← $id)
+
+
+
+namespace Term
+
+/-- Creates a value term. -/
+def mkValue [A : ValueToTerm α] : (value : α) → Env (Term α) := A.valueToTerm
+
+/-- Retrieves the value of a term. -/
+def getValue [A : TermToValue α] : Term α → Env α := A.termToValue
+
+@[inherit_doc getValue]
+def getValueAs (α : Type) [A : TermToValue α] : Term α → Env α := getValue
+
+/-- This term's sort. -/
+def getSort [ToTyp α] (term : Term α) : Env Srt := do
+  let srt' ← T.getSort term
+  let srt ← Srt.of α
+  if ¬ srt.beq srt' then throwInternal s!"expected sort {srt}, got {srt'} in term {term}"
+  return srt
+
+section variable [A : ToTyp α] [B : ToTyp β]
+
+def% mkSymbol (symbol : String) : Env (Term α) := Srt.of α >>= T.mkSymbol symbol
+
+@[inherit_doc mkSymbol]
+def mkSymbolAs (α : Type) [ToTyp α] : (symbol : String) → Env (Term α) := mkSymbol
+
+def% mkVar (symbol : String) : Env (Term α) := Srt.of α >>= T.mkVar symbol
+
+
+
+/-! ## Substitution -/
+section open Cvc.Untyped.Term renaming Subst → S
+
+/-- `Srt`-preserving substitution specification. -/
+structure Subst extends toUntyped : S where private ofUntyped ::
+
+namespace Subst
+
+@[inherit_doc S.SameSize]
+abbrev SameSize (ts1 ts2 : Terms α) (β : Type) :=
+  (same_size : ts1.size = ts2.size :=
+    by (try assumption) <;> (try grind) <;> fail "failed to prove term arrays have the same size")
+  → β
+
+@[inherit_doc S.mk]
+def mk (terms : Terms α) (replacements : Terms α) : SameSize terms replacements Subst :=
+  (ofUntyped <| S.mk terms replacements ·)
+
+@[inherit_doc S.mkOne]
+def mkOne (term : Term α) (replacement : Term α) : Subst := ofUntyped <| S.mkOne term replacement
+
+@[inherit_doc S.empty]
+def empty : Subst := ofUntyped S.empty
+
+@[inherit_doc S.push]
+def push (s : Subst) (term : Term α) (replacement : Term α) : Subst :=
+  S.push s.toUntyped term replacement |> ofUntyped
+
+@[inherit_doc S.extend]
+def extend (s : Subst) (terms : Terms α) (replacements : Terms α)
+: SameSize terms replacements Subst :=
+  (ofUntyped <| s.toUntyped.extend terms replacements ·)
+
+end Subst
+
+end
+
+@[inherit_doc T.substitute]
+def substitute (term : Term α) (subst : Subst) : Env (Term α) := T.substitute term subst.toUntyped
+
+
+
+/-! ## Polymorphic -/
+
+section poly
+
+def% equal : (lft rgt : Term α) → Env (Term Bool)
+def% @ equalN :
+  (terms : Terms α)
+  → (atLeastTwoElements : 1 < terms.size := by
+    (try grind) <;> fail "failed to prove term array has at least two elements")
+  → Env (Term Bool)
+def% equalN' : (terms : Terms α) → Env (Term Bool)
+
+def ite (cnd : Term Bool) (thn els : Term α) : Env (Term α) := T.ite cnd thn els
+
+end poly
+
+
+
+/-! ## Bool -/
+
+section bool
+
+def not (t : Term Bool) : Env (Term Bool) := T.not t
+
+def and (lft rgt : Term Bool) : Env (Term Bool) := T.and lft rgt
+def andN (terms : Terms Bool)
+  (atLeastTwoElements : 1 < terms.size := by
+    (try grind) <;> fail "failed to prove term array has at least two elements")
+: Env (Term Bool) :=
+  T.andN terms (atLeastTwoElements := atLeastTwoElements)
+def andN' (terms : Terms Bool) : Env (Term Bool) := T.andN' terms
+
+def or (lft rgt : Term Bool) : Env (Term Bool) := T.or lft rgt
+def orN (terms : Terms Bool)
+  (atLeastTwoElements : 1 < terms.size := by
+    (try grind) <;> fail "failed to prove term array has at least two elements")
+: Env (Term Bool) :=
+  T.orN terms (atLeastTwoElements := atLeastTwoElements)
+def orN' (terms : Terms Bool) : Env (Term Bool) := T.orN' terms
+
+end bool
+
+
+
+/-! ## Arithmetic -/
+
+section variable [IsArith α]
+
+def neg (t : Term Int) : Env (Term Int) := T.neg t
+
+def lt (lft rgt : Term α) : Env (Term Bool) := T.lt lft rgt
+def ltN (terms : Terms α)
+  (atLeastTwoElements : 1 < terms.size := by
+    (try grind) <;> fail "failed to prove term array has at least two elements")
+: Env (Term Bool) :=
+  T.ltN terms (atLeastTwoElements := atLeastTwoElements)
+def le (lft rgt : Term α) : Env (Term Bool) := T.le lft rgt
+def leN (terms : Terms α)
+  (atLeastTwoElements : 1 < terms.size := by
+    (try grind) <;> fail "failed to prove term array has at least two elements")
+: Env (Term Bool) :=
+  T.leN terms (atLeastTwoElements := atLeastTwoElements)
+def gt (lft rgt : Term α) : Env (Term Bool) := T.gt lft rgt
+def gtN (terms : Terms α)
+  (atLeastTwoElements : 1 < terms.size := by
+    (try grind) <;> fail "failed to prove term array has at least two elements")
+: Env (Term Bool) :=
+  T.gtN terms (atLeastTwoElements := atLeastTwoElements)
+def ge (lft rgt : Term α) : Env (Term Bool) := T.ge lft rgt
+def geN (terms : Terms α)
+  (atLeastTwoElements : 1 < terms.size := by
+    (try grind) <;> fail "failed to prove term array has at least two elements")
+: Env (Term Bool) :=
+  T.geN terms (atLeastTwoElements := atLeastTwoElements)
+
+def add (lft rgt : Term α) : Env (Term α) := T.add lft rgt
+def addN (terms : Terms α)
+  (atLeastTwoElements : 1 < terms.size := by
+    (try grind) <;> fail "failed to prove term array has at least two elements")
+: Env (Term α) :=
+  T.addN terms (atLeastTwoElements := atLeastTwoElements)
+def addN' (terms : Terms α) : Env (Term α) := T.addN' terms
+
+end
+
+
+
+/-! ## Concat-enable -/
+section variable [inst : HasConcat α]
+
+def concatN (terms : Terms α) (at_least_two : 1 < terms.size := by grind) : Env (Term α) := do
+  let valid := inst.valid_typ
+  let h_typ := Typ.typs_of_hasConcat valid
+  by
+    simp [Typ.hasConcat] at valid
+    cases h : ToTyp.typ α <;> try (
+      rw [h] at h_typ
+      revert h_typ
+      simp
+      grind only
+    )
+    case string => exact Untyped.Term.stringConcatN terms at_least_two
+    case seq _ => exact Untyped.Term.seqConcatN terms at_least_two
+
+def concat (lft rgt : Term α) : Env (Term α) := concatN #[lft, rgt]
+
+end
+
+
+
+def mkBool : Bool → Env (Term Bool) := T.mkValue
+def getBoolValue : Term Bool → Env Bool := T.getValue
+
+instance : SrtLike Bool where valueToTerm := mkBool ; termToValue := getBoolValue
+
+def mkInt : Int → Env (Term Int) := T.mkValue
+def getIntValue : Term Int → Env Int := T.getValue
+
+instance : SrtLike Int where valueToTerm := mkInt ; termToValue := getIntValue
+
+def mkRat : Rat → Env (Term Rat) := T.mkValue
+def getRatValue : Term Rat → Env Rat := T.getValue
+
+instance : SrtLike Rat where valueToTerm := mkRat ; termToValue := getRatValue
+
+def mkString : String → Env (Term String) := T.mkValue
+def getStringValue : Term String → Env String := T.getValue
+
+instance : SrtLike String where valueToTerm := mkString ; termToValue := getStringValue
+
+def mkRegex : Regex → Env (Term Regex) := T.mkValue
+def getRegexValue : Term Regex → Env Regex := T.getValue
+
+instance : SrtLike Regex where valueToTerm := mkRegex ; termToValue := getRegexValue
+
+def mkRoundingMode : Float.RoundingMode → Env (Term Float.RoundingMode) := T.mkValue
+def getRoundingModeValue : Term Float.RoundingMode → Env Float.RoundingMode := T.getValue
+
+instance : SrtLike Float.RoundingMode where
+  valueToTerm := mkRoundingMode
+  termToValue := getRoundingModeValue
+
+def mkBitVec : (BitVec size) → Env (Term (BitVec size)) := T.mkValue
+def getBitVecValue : Term (BitVec size) → Env (BitVec size) := T.getValue
+
+instance : SrtLike (BitVec size) where valueToTerm := mkBitVec ; termToValue := getBitVecValue
+
+
+
+/-! ## Sequences -/
+section sequences
+
+protected abbrev Seq (α : Type) := Term (Array α)
+
+def mkSeq [ToTyp α] [A : ValueToTerm α] : (seq : Array α) → Env (Term.Seq α) :=
+  have : Untyped.ValueToTerm α := ⟨A.valueToTerm⟩
+  T.mkValue
+
+def getSeqValue [A : TermToValue α] : Term.Seq α → Env (Array α) :=
+  have : Untyped.TermToValue α := ⟨A.termToValue⟩
+  T.getValue
+
+instance [ToTyp α] [ValueToTerm α] : ValueToTerm (Array α) := ⟨mkSeq⟩
+instance [TermToValue α] : TermToValue (Array α) := ⟨getSeqValue⟩
+
+def mkEmptySeq [A : ToTyp α] : Env (Term.Seq α) :=
+  Srt.of α >>= T.mkEmptySeq
+
+def mkEmptySeq' (α : Type) [A : ToTyp α] : Env (Term.Seq α) := mkEmptySeq
+
+def unitSeq (elem : Term α) : Env (Term.Seq α) :=
+  T.unitSeq elem
+
+def unitSeqOfValue [ToTyp α] [A : ValueToTerm α] (elem : α) : Env (Term.Seq α) :=
+  mkValue elem >>= unitSeq
+
+def mkSeqConcat (seqs : Terms (Array α)) (nempty : 0 < seqs.size := by grind) : Env (Term α) :=
+  T.mkSeqConcat seqs nempty
+
+def seqConcat (seq1 seq2 : Term.Seq α) : Env (Term.Seq α) := T.seqConcat seq1 seq2
+
+def seqPush [ToTyp α] (seq : Term.Seq α) (elem : Term α) : Env (Term.Seq α) :=
+  T.seqPush seq elem
+
+def seqPushValue [ToTyp α] [A : ValueToTerm α] (seq : Term.Seq α) (elem : α) : Env (Term α) :=
+  mkValue elem >>= seq.seqPush
+
+@[inherit_doc T.seqAt]
+def seqAt [ToTyp α] (seq : Term.Seq α) (idx : Term Int) : Env (Term.Seq α) :=
+  T.seqAt seq idx
+
+end sequences
