Cvc/Typed/Types/FiniteField.lean
@@ -1,0 +1,27 @@
+module
+
+import all Cvc.Typed.Term
+
+public import Cvc.Untyped.Types.FiniteField
+public import Cvc.Typed.Defs
+
+
+
+namespace Cvc public section variable [Ω]
+
+namespace Typed
+export Cvc (FiniteField)
+end Typed
+
+open Typed
+
+namespace FiniteField variable [Ord α] [ToTyp α]
+
+def toTypedTerm : (elem : FiniteField size) → Env (Term (FiniteField size)) :=
+  FiniteField.toTerm
+instance : ValueToTerm (FiniteField size) := ⟨toTypedTerm⟩
+
+def ofTypedTerm : Term (FiniteField size) → Env (FiniteField size) := FiniteField.ofTerm
+instance : TermToValue (FiniteField size) := ⟨ofTypedTerm⟩
+
+end FiniteField
