Cvc/Typed/Types/Float.lean
@@ -1,0 +1,27 @@
+module
+
+import all Cvc.Typed.Term
+
+public import Cvc.Untyped.Types.Float
+public import Cvc.Typed.Defs
+
+
+
+namespace Cvc public section variable [Ω]
+
+namespace Typed
+export Cvc (Float)
+end Typed
+
+open Typed
+
+namespace Float variable [Ord α] [ToTyp α]
+
+def toTypedTerm : (elem : Float exp sig) → Env (Term (Float exp sig)) :=
+  Float.toTerm
+instance : ValueToTerm (Float exp sig) := ⟨toTypedTerm⟩
+
+def ofTypedTerm : Term (Float exp sig) → Env (Float exp sig) := Float.ofTerm
+instance : TermToValue (Float exp sig) := ⟨ofTypedTerm⟩
+
+end Float
