Cvc/Untyped/Defs.lean
@@ -1,0 +1,318 @@
+/-
+Copyright (c) 2025 by the authors listed in the file AUTHORS and their
+institutional affiliations. All rights reserved.
+Released under Apache 2.0 license as described in the file LICENSE.
+Authors: Adrien Champion
+-/
+
+module
+
+public meta import Lean.Elab.BuiltinCommand
+
+public import Cvc.Basic.Env
+
+
+
+namespace Cvc
+
+
+
+public meta section codeGen open Lean Syntax Elab Command
+
+structure TypeGen where mk' ::
+  mainId : Ident
+  tParam? : Option Ident
+  subId : Ident
+  ofSubId : Ident
+  toSubId : Ident
+  idTerm : Term
+  idSig : Term
+  idDef : Term
+
+namespace TypeGen variable (tg : TypeGen)
+
+def mk (mainId : Ident) (subId : Ident)  (tParam? ofSubId? toSubId? : Option Ident)
+: CommandElabM TypeGen := do
+  let mut ofSubId := mkIdent `ofUnsafe
+  let mut toSubId := mkIdent `toUnsafe
+  if let (some ofSubId', some toSubId') := (ofSubId?, toSubId?) then
+    ofSubId := ofSubId'
+    toSubId := toSubId'
+  let mut idDef ← `($subId)
+  let mut idSig ← ``(Type)
+  let mut idTerm ← `($mainId)
+  if let some tParam := tParam? then
+    idDef ← `(fun _ => $idDef)
+    idSig ← `( (_ : Type) → $idSig )
+    idTerm ← `($idTerm $tParam)
+  return {
+    mainId, tParam?, subId, ofSubId, toSubId
+    idTerm, idSig, idDef
+  }
+
+def namespaced (code : CommandElabM α) : CommandElabM α :=
+  Lean.Elab.Command.withNamespace tg.mainId.getId code
+
+def elaborate (stx : CommandElabM (TSyntax `command)) : CommandElabM Unit := do
+  let stx ← stx
+  elabCommand stx
+
+def elab0 : CommandElabM Unit := do
+  elaborate `(
+    @[inherit_doc $tg.subId]
+    def $tg.mainId [Ω] : $tg.idSig := $tg.idDef
+  )
+  tg.namespaced do elaborate `(
+    instance : Nonempty $tg.idTerm := inferInstanceAs (Nonempty $tg.subId)
+    @[inline] private def $tg.ofSubId : $tg.subId → $tg.idTerm := id
+    @[inline] private def $tg.toSubId : $tg.idTerm → $tg.subId := id
+  )
+
+def elab1 : CommandElabM Unit := do
+  tg.elab0
+  let toStringId := `toString |> mkIdent
+  let toStringSubId := tg.subId.getId |>.append `toString |> mkIdent
+  tg.namespaced do elaborate `(
+    instance : ToString $tg.idTerm := inferInstanceAs (ToString $tg.subId)
+    @[inherit_doc $toStringSubId]
+    protected def $toStringId : $tg.idTerm → String := $toStringSubId
+  )
+
+def elab2 : CommandElabM Unit := do
+  tg.elab1
+  let beqId := `beq |> mkIdent
+  let beqSubId := tg.subId.getId |>.append `beq |> mkIdent
+  let hashId := `hash |> mkIdent
+  let hashSubId := tg.subId.getId |>.append `hash |> mkIdent
+  tg.namespaced do elaborate `(
+    instance : BEq $tg.idTerm := inferInstanceAs (BEq $tg.subId)
+    @[inherit_doc $beqSubId]
+    protected def $beqId : $tg.idTerm → $tg.idTerm → Bool := $beqSubId
+    instance : Hashable $tg.idTerm := inferInstanceAs (Hashable $tg.subId)
+    @[inherit_doc $hashSubId]
+    protected def $hashId : $tg.idTerm → UInt64 := $hashSubId
+  )
+
+def elab3 : CommandElabM Unit := do
+  tg.elab2
+  let bltId := `blt |> mkIdent
+  let bltSrc := tg.subId.getId |>.append `blt |> mkIdent
+  let bleId := `ble |> mkIdent
+  let bleSrc := tg.subId.getId |>.append `ble |> mkIdent
+  let bgtId := `bgt |> mkIdent
+  let bgtSrc := tg.subId.getId |>.append `bgt |> mkIdent
+  let bgeId := `bge |> mkIdent
+  let bgeSrc := tg.subId.getId |>.append `bge |> mkIdent
+  let compareId := `compare |> mkIdent
+  let compareSrc := tg.subId.getId |>.append `compare |> mkIdent
+  tg.namespaced do elaborate `(
+    instance : LT $tg.idTerm := inferInstanceAs (LT $tg.subId)
+    instance : DecidableLT $tg.idTerm := inferInstanceAs (DecidableLT $tg.subId)
+    instance : LE $tg.idTerm := inferInstanceAs (LE $tg.subId)
+    instance : DecidableLE $tg.idTerm := inferInstanceAs (DecidableLE $tg.subId)
+
+    @[inherit_doc $bltSrc]
+    protected def $bltId : $tg.idTerm → $tg.idTerm → Bool := $bltSrc
+    @[inherit_doc $bleSrc]
+    protected def $bleId : $tg.idTerm → $tg.idTerm → Bool := $bleSrc
+    @[inherit_doc $bgtSrc]
+    protected def $bgtId : $tg.idTerm → $tg.idTerm → Bool := $bgtSrc
+    @[inherit_doc $bgeSrc]
+    protected def $bgeId : $tg.idTerm → $tg.idTerm → Bool := $bgeSrc
+
+    instance : Ord $tg.idTerm := inferInstanceAs (Ord $tg.subId)
+
+    @[inherit_doc $compareSrc]
+    protected def $compareId : $tg.idTerm → $tg.idTerm → Ordering := $compareSrc
+  )
+
+end TypeGen
+
+declare_syntax_cat cvcCustomDefKw
+
+syntax "def0% " : cvcCustomDefKw
+syntax "def1% " : cvcCustomDefKw
+syntax "def2% " : cvcCustomDefKw
+syntax "def3% " : cvcCustomDefKw
+
+syntax (name := cvcCustomDef)
+  cvcCustomDefKw ident (ident)? " ← " ident
+    ("( " ident " / " ident " )")?
+: command
+
+@[command_elab cvcCustomDef]
+def elab_cvcCustomDef : CommandElab
+| `( $kw:cvcCustomDefKw $id $[ $tParam? ]? ← $subId $[ ( $ofSubId? / $toSubId? ) ]? ) => do
+  let tg ← TypeGen.mk id subId tParam? ofSubId? toSubId?
+  match kw with
+  | `(cvcCustomDefKw| def0%) => tg.elab0
+  | `(cvcCustomDefKw| def1%) => tg.elab1
+  | `(cvcCustomDefKw| def2%) => tg.elab2
+  | `(cvcCustomDefKw| def3%) => tg.elab3
+  | _ => throwUnsupportedSyntax
+| _ => throwUnsupportedSyntax
+
+end codeGen
+
+
+public section variable [Ω]
+
+def0% Proof ← cvc5.Proof
+
+def1% Command ← cvc5.Command
+
+def2% Datatype.Decl ← cvc5.DatatypeDecl
+def2% Datatype ← cvc5.Datatype
+def2% Datatype.Constructor.Decl ← cvc5.DatatypeConstructorDecl
+def2% Datatype.Constructor ← cvc5.DatatypeConstructor
+def2% Datatype.Selector ← cvc5.DatatypeSelector
+def2% Grammar ← cvc5.Grammar
+
+
+
+def3% Srt ← cvc5.Sort
+
+namespace Srt
+
+inductive Abstract
+| array
+| bitVec
+| float
+| finiteField
+| function
+| bag
+| set
+| seq
+deriving Inhabited, DecidableEq, BEq, Ord, Hashable, Repr
+
+namespace Abstract
+
+protected def toString : (a : Srt.Abstract) → String
+| array => "Array _ _"
+| bitVec => "BitVec _"
+| float => "Float _ _"
+| finiteField => "FiniteField _"
+| function => "_ → _"
+| bag => "Bag _"
+| set => "Set _"
+| seq => "Seq _"
+
+instance : ToString Srt.Abstract := ⟨Abstract.toString⟩
+
+private def ofKind : (k : cvc5.SortKind) → Res Abstract
+  | .ARRAY_SORT => return array
+  | .BITVECTOR_SORT => return bitVec
+  | .FLOATINGPOINT_SORT => return float
+  | .FINITE_FIELD_SORT => return finiteField
+  | .FUNCTION_SORT => return function
+  | .BAG_SORT => return bag
+  | k => throwInternal s!"sort kind `{k}` is not abstract-able"
+
+def toKind : (a : Abstract) → cvc5.SortKind
+  | array => .ARRAY_SORT
+  | bitVec => .BITVECTOR_SORT
+  | float => .FLOATINGPOINT_SORT
+  | finiteField => .FINITE_FIELD_SORT
+  | function => .FUNCTION_SORT
+  | bag => .BAG_SORT
+  | set => .SET_SORT
+  | seq => .SEQUENCE_SORT
+
+instance : Ord Abstract := ⟨fun a1 a2 => compare a1.ctorIdx a2.ctorIdx⟩
+
+section variable (a1 a2 : Abstract)
+
+protected def ble : Bool := a1.ctorIdx ≤ a2.ctorIdx
+protected def blt : Bool := a1.ctorIdx < a2.ctorIdx
+
+end
+
+instance : LE Abstract := ⟨(Abstract.ble · ·)⟩
+instance : DecidableLE Abstract := fun a1 a2 => if h : a1.ble a2 then isTrue h else isFalse h
+instance : LT Abstract := ⟨(Abstract.blt · ·)⟩
+instance : DecidableLT Abstract := fun a1 a2 => if h : a1.blt a2 then isTrue h else isFalse h
+
+end Abstract
+end Srt
+
+/-- An array of `Srt`s. -/
+abbrev Srts := Array Srt
+
+namespace Srts
+
+private def toUnsafe : Srts → Array cvc5.Sort := id
+private def ofUnsafe : Array cvc5.Sort → Srts := id
+
+end Srts
+
+
+
+inductive Typ
+| bool | int | real | string | regex | roundingMode
+| bitVec (size : Nat)
+| float (exp sig : Nat)
+| finiteField (size : Nat)
+| arrayTo (idx elm : Typ)
+| bag (elm : Typ) | set (elm : Typ) | seq (elm : Typ)
+| abstract (a : Srt.Abstract)
+| function (dom : Typ) (cod : Typ)
+deriving DecidableEq, Ord, Hashable
+
+namespace Typ
+
+protected def toString (t : Typ) (paren : Bool := false) : String :=
+  let paren (s : String) := if paren then s!"({s})" else s
+  match t with
+  | bool => "Bool" | int => "Int" | real => "Real" | string => "String"
+  | regex => "Regex" | roundingMode => "RoundingMode"
+  | bitVec size => paren s!"BitVec {size}"
+  | float exp sig => paren s!"Float {exp} {sig}"
+  | finiteField size => paren s!"FiniteField {size}"
+  | arrayTo idx elm => paren s!"Array {idx.toString true} {elm.toString true}"
+  | bag elm => paren s!"Bag {elm.toString true}"
+  | set elm => paren s!"Set {elm.toString true}"
+  | seq elm => paren s!"Seq {elm.toString true}"
+  | abstract a => paren s!"Abstract {a}"
+  | function dom cod => paren s!"{dom.toString false} → {cod.toString false}"
+
+instance : ToString Typ := ⟨Typ.toString⟩
+
+end Typ
+
+class ToTyp (α : Type) where
+  /-- `Typ` associated to a type through `ToTyp`. -/
+  typ : Typ
+
+
+
+namespace Untyped
+
+def3% Term ← cvc5.Term
+
+/-- An array of `Srt`s. -/
+abbrev Terms := Array Term
+
+namespace Terms
+
+private def toUnsafe : Terms → Array cvc5.Term := id
+private def ofUnsafe : Array cvc5.Term → Terms := id
+
+end Terms
+
+class TermToValue (α : Type) where
+  termToValue : Term → Env α
+
+namespace TermToValue
+instance : TermToValue Term := ⟨pure⟩
+end TermToValue
+
+class ValueToTerm (α : Type) where
+  valueToTerm : α → Env Term
+
+namespace ValueToTerm
+instance : ValueToTerm Term := ⟨pure⟩
+end ValueToTerm
+
+class abbrev SrtLike (α : Type) := ToTyp α, TermToValue α, ValueToTerm α
+
+end Untyped
