Cvc/Untyped/Solver.lean
@@ -1,0 +1,435 @@
+/-
+Copyright (c) 2026 by the authors listed in the file AUTHORS and their
+institutional affiliations. All rights reserved.
+Released under Apache 2.0 license as described in the file LICENSE.
+Authors: Adrien Champion
+-/
+
+module
+
+import all Cvc.Basic
+import all Cvc.Untyped.Term
+
+public import Cvc.Basic
+public import Cvc.Logic
+public import Cvc.Untyped.Defs
+
+
+
+namespace Cvc.Untyped public section
+
+
+
+
+def Solver [Ω] := cvc5.Solver
+
+/-! ## Solver-mode monadic environment -/
+section variable [Ω] [Monad m]
+
+local macro "env_gen% " envT:ident " / " env:ident : command =>
+  let pureId := Lean.mkIdent `pure
+  let bindId := Lean.mkIdent `bind
+  let throwId := Lean.mkIdent `throw
+  let tryCatchId := Lean.mkIdent `tryCatch
+  let baseIOIdent := Lean.mkIdent ``BaseIO
+  `(
+abbrev $env := $envT $baseIOIdent
+
+namespace $envT variable {α β : Type} {m : Type → Type} [Monad m]
+
+protected def $pureId (a : α) : $envT m α := ⟨return a⟩
+protected def $bindId (a : $envT m α) (f : α → $envT m β) : $envT m β :=
+  ⟨a.toEnv.bind (fun a => f a |>.toEnv)⟩
+
+instance [Monad m] : Monad ($envT m) where
+  pure := .$pureId
+  bind := .$bindId
+
+protected def $throwId (e : Error) : $envT m α := ⟨throw e⟩
+protected def $tryCatchId (code : $envT m α) (errorDo : Error → $envT m α) : $envT m α :=
+  ⟨code.toEnv.tryCatch fun e => errorDo e |>.toEnv⟩
+
+instance : MonadExcept Error ($envT m) where
+  throw := .$throwId
+  tryCatch := .$tryCatchId
+
+def transformLift (code : m α) : $envT m α :=
+  ⟨code⟩
+
+instance : MonadLift m ($envT m) := ⟨transformLift⟩
+
+/-- Lifts `EnvT`-code.
+
+‼️ dangerous: allows performing check-sat-s, thus changing  -/
+private def lift : EnvT m α → $envT m α := .wrap
+
+private instance : MonadLift (EnvT m) ($envT m) := ⟨lift⟩
+
+def liftMonadVersion [Monad m] [MonadLiftT BaseIO m] (code : $env α) : $envT m α :=
+  ⟨liftM code.toEnv⟩
+instance [Monad m] [MonadLiftT BaseIO m] : MonadLift $env ($envT m) := ⟨liftMonadVersion⟩
+end $envT
+  )
+
+structure EnvSatT [Ω] (m : Type → Type) (α : Type) where
+private wrap ::
+  private toEnv : EnvT m α
+
+env_gen% EnvSatT / EnvSat
+
+structure EnvUnsatT (m : Type → Type) (α : Type) where
+private wrap ::
+  private toEnv : EnvT m α
+
+env_gen% EnvUnsatT / EnvUnsat
+
+structure EnvUnknownT (m : Type → Type) (α : Type) where
+private wrap ::
+  private toEnv : EnvT m α
+
+env_gen% EnvUnknownT / EnvUnknown
+
+
+
+namespace Solver variable [Ω] open cvc5 renaming TermManager → Tm, Solver → S
+
+/-- Creates a new solver. -/
+def new : Env Solver := runUnsafe (S.new ·)
+
+section variable [MonadLiftT BaseIO m] (s : Solver)
+
+/-- Conversion to cvc5. -/
+private def toUnsafe : S := s
+
+
+
+def Result := cvc5.Result
+
+namespace Result
+
+private def toUnsafe : Result → cvc5.Result := id
+private def ofUnsafe : cvc5.Result → Result := id
+
+section variable (r : Result)
+
+protected def toString : String := r.toUnsafe.toString
+instance : ToString Result := ⟨Result.toString⟩
+
+private def isSat! : Bool := r.toUnsafe.isSat
+private def isUnsat! : Bool := r.toUnsafe.isUnsat
+private def isUnknown! : Bool := r.toUnsafe.isUnknown
+private def getUnknownExplanation? : Option Unknown.Explanation :=
+  r.toUnsafe.getUnknownExplanation? |>.map Unknown.Explanation.ofUnsafe
+
+abbrev Sat? := Bool ⊕ Unknown.Explanation
+
+def isSat? : Res Sat? :=
+  if r.isSat then return .inl true
+  else if r.isUnsat then return .inl false
+  else if let some unkExpl := r.getUnknownExplanation? then return .inr unkExpl
+  else throwInternal s!"check result is neither sat, unsat, or unknown\n{r}"
+
+def isSat : Res Bool := r.isSat? >>= fun
+  | .inl res => return res
+  | .inr unkExpl => throwUser s!"unexpected unknown result: {unkExpl}"
+
+
+end
+
+end Result
+
+
+
+@[inherit_doc S.getVersion]
+def getVersion : Env String := runUnsafe' do
+  s.toUnsafe.getVersion
+
+@[inherit_doc S.setOption]
+def setOption (option value : String) : Env Unit := runUnsafe' do
+  s.toUnsafe.setOption option value
+
+@[inherit_doc S.getOption]
+def getOption (flag : String) : Env String := runUnsafe' do
+  s.toUnsafe.getOption flag
+
+@[inherit_doc S.getOptionNames]
+def getOptionNames : Env (Array String) := runUnsafe' do
+  s.toUnsafe.getOptionNames
+
+@[inherit_doc S.setInfo]
+def setInfo (option value : String) : Env Unit := runUnsafe' do
+  s.toUnsafe.setInfo option value
+
+@[inherit_doc S.getInfo]
+def getInfo (flag : String) : Env String := runUnsafe' do
+  s.toUnsafe.getInfo flag
+
+@[inherit_doc S.setLogic]
+def setLogic (logic : Logic) : Env Unit := runUnsafe' do
+  s.toUnsafe.setLogic logic.toSmtLib
+
+@[inherit_doc S.isLogicSet]
+def isLogicSet : Env Bool := runUnsafe' do
+  s.toUnsafe.isLogicSet
+
+@[inherit_doc S.getLogic]
+def getLogicString : Env String := runUnsafe' do
+  s.toUnsafe.getLogic
+
+@[inherit_doc S.getLogic]
+def getLogic : Env Logic := s.getLogicString >>= liftM ∘ Logic.ofSmtLib
+
+@[inherit_doc S.getAssertions]
+def getAssertions : Env Terms := runUnsafe' do
+  s.toUnsafe.getAssertions
+
+@[inherit_doc S.getInstantiations]
+def getInstantiations : Env String := runUnsafe' do
+  s.toUnsafe.getInstantiations
+
+
+
+@[inherit_doc S.resetAssertions]
+def reset : Env Unit := runUnsafe' do
+  s.toUnsafe.resetAssertions
+
+@[inherit_doc S.push]
+def push (nscopes : UInt32 := 1) : Env Unit := runUnsafe' do
+  s.toUnsafe.push nscopes
+
+@[inherit_doc S.pop]
+def pop (nscopes : UInt32 := 1) : Env Unit := runUnsafe' do
+  s.toUnsafe.pop nscopes
+
+
+
+@[inherit_doc S.assertFormula]
+def assert (t : Term) : Env Unit := runUnsafe' do
+  s.toUnsafe.assertFormula t
+
+@[inherit_doc S.declareFun]
+def declareFun (symbol : String) (sorts : Srts) (sort : Srt) (fresh : Bool := true) : Env Term :=
+  runUnsafe' do s.toUnsafe.declareFun symbol sorts sort fresh
+
+/-- Declares a constant function symbol. -/
+def declareConst (symbol : String) (sort : Srt) (fresh : Bool := true) : Env Term :=
+  s.declareFun symbol #[] sort (fresh := fresh)
+
+@[inherit_doc S.declareSort]
+def declareSrt
+  (symbol : String) (arity : UInt32) (fresh : Bool := false)
+: Env Srt :=
+  runUnsafe' do s.toUnsafe.declareSort symbol arity fresh
+
+@[inherit_doc S.defineFun]
+def defineFun
+  (symbol : String) (boundVars : Terms) (sort : Srt) (body : Term) (global : Bool := false)
+: Env Term :=
+  runUnsafe' do s.toUnsafe.defineFun symbol boundVars sort body global
+
+/-- Defines a constant function symbol. -/
+def defineConst (symbol : String) (sort : Srt) (body : Term) (global : Bool := false) : Env Term :=
+  s.defineFun symbol #[] sort body (global := global)
+
+@[inherit_doc S.defineFunRec]
+def defineFunRec
+  (symbol : String) (boundVars : Terms) (sort : Srt) (body : Term) (global : Bool := false)
+: Env Term :=
+  runUnsafe' do s.toUnsafe.defineFunRec symbol boundVars sort body global
+
+@[inherit_doc S.defineFunRecTerm]
+def defineFunRecTerm
+  (fn : Term) (boundVars : Terms) (body : Term) (global : Bool := false)
+: Env Term :=
+  runUnsafe' do s.toUnsafe.defineFunRecTerm fn boundVars body global
+
+@[inherit_doc S.defineFunsRec]
+def defineFunsRec
+  (funs : Terms) (boundVars : Array Terms) (bodies : Terms) (global : Bool := false)
+: Env Unit :=
+  runUnsafe' do s.toUnsafe.defineFunsRec funs boundVars bodies global
+
+
+
+@[inherit_doc S.getQuantifierElimination]
+def qe (q : Term) : Env Term := runUnsafe' do s.toUnsafe.getQuantifierElimination q
+
+@[inherit_doc S.getQuantifierEliminationDisjunct]
+def qeDisjunct (q : Term) : Env (Option Term) := do
+  let term ← runUnsafe' do s.toUnsafe.getQuantifierEliminationDisjunct q
+  return if term.isNull then none else some term
+
+@[inherit_doc S.getInterpolant]
+def getInterpolant (conj : Term) (grammar : Option Grammar := none) : Env Term :=
+  runUnsafe' do s.toUnsafe.getInterpolant conj grammar
+
+@[inherit_doc S.getInterpolantNext]
+def getNextInterpolant : Env (Option Term) := do
+  let term ← runUnsafe' do s.toUnsafe.getInterpolantNext
+  return if term.isNull then none else some term
+
+@[inherit_doc S.getAbduct]
+def getAbduct (conj : Term) (grammar : Option Grammar := none) : Env Term :=
+  runUnsafe' do s.toUnsafe.getAbduct conj grammar
+
+@[inherit_doc S.getAbductNext]
+def getNextAbduct : Env (Option Term) := do
+  let term ← runUnsafe' do s.toUnsafe.getAbductNext
+  return if term.isNull then none else some term
+
+@[inherit_doc S.proofToString]
+def proofToString (proof : Proof)
+  (format : Proof.Format := default)
+: Env (Option String) :=
+  runUnsafe' do s.toUnsafe.proofToString proof format.toUnsafe
+
+@[inherit_doc S.getLearnedLiterals]
+def getLearnedLiterals (t : LearnedLitType := LearnedLitType.input) : Env Terms :=
+  runUnsafe' do s.toUnsafe.getLearnedLiterals t.toUnsafe
+
+
+
+section unexpected
+
+private def unexpectedResult (badResDesc : String) (dumpAssertions : Bool)
+  (explanation : Option String := none)
+: Env α := do
+  let _ := s
+  let mut msg := s!"unexpected `{badResDesc}` result"
+  if let some e := explanation then msg := s!"{msg}\n- {e}"
+  if dumpAssertions then
+    let assertions ← s.getAssertions
+    if assertions.isEmpty then
+      msg := s!"{msg}, solver does not have any assertions"
+    else
+      msg := msg ++ " for the following assertions\n```smtlib"
+        |> assertions.foldl (s!"{·}\n(assert {·})")
+      msg := msg ++ "\n```"
+  throwUser msg
+
+variable (e : Unknown.Explanation) (dumpAssertions : Bool := false)
+
+/-- Fails if `sat` was unexpected, shows all assertions if `dumpAssertions` (default false). -/
+def unexpectedSat : EnvSat α := s.unexpectedResult "sat" dumpAssertions
+/-- Fails if `unsat` was unexpected, shows all assertions if `dumpAssertions` (default false). -/
+def unexpectedUnsat : EnvUnsat α := s.unexpectedResult "unsat" dumpAssertions
+/-- Fails if `unknown` was unexpected, shows all assertions if `dumpAssertions` (default false). -/
+def unexpectedUnknown : EnvUnknown α :=
+  s.unexpectedResult "unknown" dumpAssertions (explanation := toString e)
+
+end unexpected
+
+
+
+section check_sat variable (assuming : Option Terms := none)
+
+/-- Checks the satisfiability of the constraints asserted so far. -/
+def checkSatResult : Env Result := do
+  let code := if let some terms := assuming then S.checkSatAssuming s terms else S.checkSat s
+  Result.ofUnsafe <$> runUnsafe' code
+
+@[inherit_doc checkSatResult]
+def checkIsSat? : Env Result.Sat? := do
+  let res ← s.checkSatResult assuming
+  res.isSat?
+
+@[inherit_doc checkSatResult]
+def checkIsSat : Env Bool := do
+  let res ← s.checkSatResult assuming
+  res.isSat
+
+@[inherit_doc checkSatResult]
+def checkSat
+  (ifSat : EnvSatT m α := s.unexpectedSat)
+  (ifUnsat : EnvUnsatT m α := s.unexpectedUnsat)
+  (ifUnknown : Unknown.Explanation → EnvUnknownT m α := liftM ∘ s.unexpectedUnknown)
+: EnvT m α := do
+  match ← s.checkIsSat? (assuming := assuming) with
+  | .inl true => ifSat.toEnv
+  | .inl false => ifUnsat.toEnv
+  | .inr unkExpl => ifUnknown unkExpl |>.toEnv
+
+@[inherit_doc checkSatResult]
+def checkSat? {α : Type} (s : Solver) (assuming : Option Terms := none)
+  (ifSat : EnvSatT m (Option α) := return none)
+  (ifUnsat : EnvUnsatT m (Option α) := return none)
+  (ifUnknown : Unknown.Explanation → EnvUnknownT m (Option α) := liftM ∘ s.unexpectedUnknown)
+: EnvT m (Option α) :=
+  s.checkSat assuming ifSat ifUnsat ifUnknown
+
+end check_sat
+
+
+
+section sat
+
+/-- Get the value of `term` in the current model.
+
+# TODO
+- requires model-production
+-/
+def getValue (term : Term) : EnvSat Term := runUnsafe' do s.toUnsafe.getValue term
+/-- Get the value of each term in  `terms` in the current model.
+
+# TODO
+- requires model-production
+-/
+def getValues (terms : Terms) : EnvSat Terms := runUnsafe' do s.toUnsafe.getValues terms
+
+@[inherit_doc S.getModelDomainElements]
+def getModelDomainElements (sort : Srt) : EnvSat Terms :=
+  runUnsafe' do s.toUnsafe.getModelDomainElements sort
+
+@[inherit_doc S.isModelCoreSymbol]
+def isModelCoreSymbol (term : Term) : EnvSat Bool :=
+  runUnsafe' do s.toUnsafe.isModelCoreSymbol term
+
+@[inherit_doc S.getModel]
+def getModelAsString (sorts : Srts) (consts : Terms) : EnvSat String :=
+  runUnsafe' do s.toUnsafe.getModel sorts consts
+
+@[inherit_doc S.blockModel]
+def blockModel (mode : Model.BlockMode) : EnvSat Unit :=
+  runUnsafe' do s.toUnsafe.blockModel mode.toUnsafe
+
+@[inherit_doc S.blockModelValues]
+def blockModelValues (terms : Terms) : EnvSat Unit :=
+  runUnsafe' do s.toUnsafe.blockModelValues terms
+
+end sat
+
+
+
+section unsat
+
+@[inherit_doc S.getUnsatAssumptions]
+def getUnsatAssumptions: EnvUnsat Terms := runUnsafe' do s.toUnsafe.getUnsatAssumptions
+
+@[inherit_doc S.getProof]
+def getUnsatProof (c : Proof.Component := Proof.Component.full) : EnvUnsat (Array Proof) :=
+  runUnsafe' do s.toUnsafe.getProof c.toUnsafe
+
+@[inherit_doc S.getUnsatCore]
+def getUnsatCore : EnvUnsat Terms := runUnsafe' do s.toUnsafe.getUnsatCore
+
+@[inherit_doc S.getUnsatCoreLemmas]
+def getUnsatCoreLemmas : EnvUnsat Terms := runUnsafe' do s.toUnsafe.getUnsatCoreLemmas
+
+end unsat
+
+
+
+section unknown
+
+@[inherit_doc S.getTimeoutCore]
+def getTimeoutCore : EnvUnknown (cvc5.Result × Terms) := runUnsafe' do s.toUnsafe.getTimeoutCore
+
+@[inherit_doc S.getTimeoutCoreAssuming]
+def getTimeoutCoreAssuming (assumptions : Terms) : EnvUnknown (cvc5.Result × Terms) :=
+  runUnsafe' do s.toUnsafe.getTimeoutCoreAssuming assumptions
+
+end unknown
+
+end
+
+end Solver
