Cvc/Untyped/Term.lean
@@ -1,0 +1,520 @@
+/-
+Copyright (c) 2026 by the authors listed in the file AUTHORS and their
+institutional affiliations. All rights reserved.
+Released under Apache 2.0 license as described in the file LICENSE.
+Authors: Adrien Champion
+-/
+
+module
+
+import all Cvc.Basic.Env
+import all Cvc.Untyped.Defs
+import all Cvc.Untyped.Srt
+
+public import Cvc.Untyped.Srt
+import Lean.Parser.Term
+
+
+
+namespace Cvc public section open cvc5 renaming TermManager → Tm, Term → T variable [Ω]
+
+local macro "lift% " fn:ident args:(ppSpace term:max)* : term =>
+  `((runUnsafe fun tm =>tm.$fn $[ $args]* : Env Untyped.Term))
+
+local macro "liftKind% " op:term:max args:(ppSpace term:max)* : term =>
+  `((runUnsafe fun tm =>tm.mkTerm $op #[$[ $args],*] : Env Untyped.Term))
+
+
+local macro "def% " id:ident args:(ppSpace ident)* " := " fn:ident : command =>
+  let fnId := ``Tm |>.append fn.getId |> Lean.mkIdent
+  `(@[inherit_doc $fnId] def $id := fun $[ $args]* => (lift% $fn $[ $args]* : Env Untyped.Term))
+
+
+
+
+namespace Untyped.Term
+
+/-- Creates a constant value. -/
+def mkValue [A : ValueToTerm α] : (value : α) → Env Term := A.valueToTerm
+@[inherit_doc mkValue]
+def mkValueAs (α : Type) [A : ValueToTerm α] : (value : α) → Env Term := mkValue
+
+/-- Extracts an `α`-value from a constant term. -/
+def getValue [A : TermToValue α] : Term → Env α := A.termToValue
+
+@[inherit_doc getValue]
+def getValueAs (α : Type) [A : TermToValue α] : Term → Env α := getValue
+
+
+
+def% mkBool b := mkBoolean
+def% mkInt i := mkInteger
+def% mkReal r := mkRealOfRat
+def% mkRealOfString s := mkRealOfString
+
+@[inherit_doc Tm.mkConst]
+def mkSymbolOfSrt (srt : Srt) (symbol : String) : Env Term := lift% mkConst srt symbol
+
+@[inherit_doc Tm.mkConst]
+def mkSymbol (symbol : String) (srt : Srt) : Env Term := mkSymbolOfSrt srt symbol
+
+@[inherit_doc Tm.mkConst]
+def mkSymbolAs (α : Type) [ToTyp α] (symbol : String) : Env Term :=
+  Srt.of α >>= mkSymbol symbol
+
+@[inherit_doc Tm.mkVar]
+def mkVar (symbol : String) (srt : Srt) : Env Term := lift% mkVar srt symbol
+
+@[inherit_doc Tm.mkString]
+def mkString (s : String) (useEscSequences : Bool := false) : Env Term :=
+  lift% mkString s useEscSequences
+
+@[inherit_doc Tm.mkRoundingMode]
+def mkRoundingMode (rm : Float.RoundingMode) : Env Term := lift% mkRoundingMode rm.toUnsafe
+
+instance : Untyped.ValueToTerm Float.RoundingMode := ⟨mkRoundingMode⟩
+
+@[inherit_doc Tm.mkBitVector]
+def mkConstBitVec (size : UInt32) (val : UInt64 := 0) : Env Term := lift% mkBitVector size val
+
+@[inherit_doc Tm.mkBitVectorOfString]
+def mkBitVecOfString (size : UInt32) (s : String) (base : BitVec.Base := .bin) : Env Term :=
+  lift% mkBitVectorOfString size s base.toUInt32
+
+def mkBitVec (bv : BitVec size) : Env Term := mkConstBitVec size.toUInt32 bv.toNat.toUInt64
+
+@[inherit_doc Tm.mkFloatingPoint]
+def mkFloatOfBitVec (exp sig : UInt32) (bv : Term) : Env Term :=
+  lift% mkFloatingPoint exp sig bv
+
+@[inherit_doc Tm.mkFloatingPointPosInf]
+def mkFloatPosInf (exp sig : UInt32) : Env Term :=
+  lift% mkFloatingPointPosInf exp sig
+
+@[inherit_doc Tm.mkFloatingPointNegInf]
+def mkFloatNegInf (exp sig : UInt32) : Env Term :=
+  lift% mkFloatingPointNegInf exp sig
+
+@[inherit_doc Tm.mkFloatingPointNaN]
+def mkFloatNaN (exp sig : UInt32) : Env Term :=
+  lift% mkFloatingPointNaN exp sig
+
+@[inherit_doc Tm.mkFloatingPointPosZero]
+def mkFloatPosZero (exp sig : UInt32) : Env Term :=
+  lift% mkFloatingPointPosZero exp sig
+
+@[inherit_doc Tm.mkFloatingPointNegZero]
+def mkFloatNegZero (exp sig : UInt32) : Env Term :=
+  lift% mkFloatingPointNegZero exp sig
+
+@[inherit_doc Tm.mkFiniteFieldElem]
+def mkFiniteFieldElemOfValue (value : Int) (sort : Srt) : Env Term :=
+  lift% mkFiniteFieldElem value sort
+
+/-- The array that associates a default value to all indices.
+
+- `srt`: the sort of the array being constructed, must be an array-sort.
+- `default`: the default value all indices map to.
+-/
+def mkArray (srt : Srt) (default : Term) : Env Term := lift% mkConstArray srt default
+
+/-- The empty set for set-sort `srt`. -/
+def mkEmptySet (srt : Srt) := lift% mkEmptySet srt
+
+/-- Set insertion. -/
+def setInsert (set elem : Term) : Env Term := liftKind% .SET_INSERT set elem
+
+section sequences
+/-- The empty sequence with `srt` elements. -/
+def mkEmptySeq (srt : Srt) := lift% mkEmptySequence srt
+
+/-- Creates a sequence with one element. -/
+def unitSeq (elm : Term) := liftKind% .SEQ_UNIT elm
+
+/-- Sequence concatenation. -/
+def mkSeqConcat (seqs : Terms) : (nempty : 0 < seqs.size := by grind) → Env Term := fun _ => do
+  let seqs ← seqs.mapM unitSeq
+  runUnsafe fun tm => tm.mkTerm .SEQ_CONCAT seqs
+
+def seqConcatN (seqs : Terms)
+: (at_least_2 : 1 < seqs.size := by grind) → Env Term := fun _ => do
+  runUnsafe fun tm => tm.mkTerm .SEQ_CONCAT seqs
+
+@[inherit_doc mkSeqConcat]
+def seqConcat (seq1 seq2 : Term) : Env Term := liftKind% .SEQ_CONCAT seq1 seq2
+
+def seqLength (seq : Term) : Env Term := liftKind% .SEQ_LENGTH seq
+
+/-- Sequence indexing -/
+def seqAt (seq idx : Term) : Env Term := liftKind% .SEQ_AT seq idx
+
+/-- Adds an element at the end of a sequence. -/
+def seqPush (seq elem : Term) : Env Term := elem.unitSeq >>= seq.seqConcat
+
+def mkSeqValue [ToTyp α] [ValueToTerm α] (elems : Array α) : Env Term := do
+  let elems ← elems.mapM mkValue
+  if h : 0 < elems.size then mkSeqConcat elems
+  else Srt.of α >>= mkEmptySeq
+
+end sequences
+
+section bags
+/-- The empty bag for bag-sort `srt`. -/
+def mkEmptyBag (srt : Srt) := lift% mkEmptyBag srt
+
+/-- Creates a bag where `elem` maps to `count`. -/
+def mkBagWith (elem count : Term) := liftKind% .BAG_MAKE elem count
+
+/-- Creates the term for the count of `elem` in `bag`. -/
+def bagCount (bag elem : Term) := liftKind% .BAG_COUNT bag elem
+
+/-- Max-union between bag-terms. -/
+def bagUnionMax (bag1 bag2 : Term) := liftKind% .BAG_UNION_MAX bag1 bag2
+/-- Disjoint-union between bag-terms. -/
+def bagUnionDisjoint (bag1 bag2 : Term) := liftKind% .BAG_UNION_DISJOINT bag1 bag2
+/-- Min-intersection between bag-terms. -/
+def bagInterMin (bag1 bag2 : Term) := liftKind% .BAG_INTER_MIN bag1 bag2
+end bags
+
+
+
+
+/-! ## Operators -/
+
+
+
+/-! ### `Bool` operators -/
+
+open Lean open Parser.Command (docComment) in
+
+/-- Creates a `docComment` syntax node from a `String` docstring. -/
+public meta def mkDocComment (s : String) : TSyntax ``docComment :=
+  Lean.mkNode ``docComment #[mkAtom "/--", mkAtom (s ++ "-/")]
+
+declare_syntax_cat def_2nary_defaults
+
+syntax ", " "(" term ", " term ")" : def_2nary_defaults
+
+local macro
+  mods:declModifiers
+  "def_2nary% " id:ident " := " kind:term defaults?:optional(def_2nary_defaults)
+: command => do
+  let (rawId, rawIdN, idN, rawIdN', idN') ← match id.getId with
+    | .str base s =>
+      let rawIdN := s!"{s}N"
+      let rawIdN' := s!"{s}N'"
+      pure (
+        s,
+        rawIdN, Lean.Name.str base rawIdN |> Lean.mkIdent,
+        rawIdN', Lean.Name.str base rawIdN' |> Lean.mkIdent,
+      )
+    | _ => Lean.Macro.throwError ""
+  let cmt := Id.run do
+    let mut cmt := s!"N-ary version of `{rawId}`, requires at least two elements"
+    if defaults?.isSome
+    then cmt := s!"{cmt}; see also `{rawIdN'}`."
+    else cmt := cmt ++ "."
+    mkDocComment cmt
+  let termsId := `terms |> mkIdent
+  let validId := `atLeastTwoElements |> mkIdent
+  let mainDefs ← `(
+    $mods:declModifiers
+    def $id (t1 t2 : Term) : Env Term := liftKind% $kind t1 t2
+    $cmt:docComment
+    def $idN ($termsId : Terms)
+      ($validId : 2 ≤ $(termsId).size := by
+        (try grind) <;> fail "failed to prove term array has at least two elements")
+    : Env Term :=
+      let _ := $validId
+      lift% mkTerm $kind $termsId
+  )
+  if let some defaults := defaults? then
+    match defaults with
+    | `(def_2nary_defaults| , ( $on0:term , $on1:term ) ) =>
+      let cmt' := mkDocComment
+        s!"N-ary version of `{rawId}` with defaults for zero- and one-element arrays; \
+        see also `{rawIdN}`."
+      `(
+        $mainDefs
+        $cmt':docComment
+        def $idN' (terms : Terms)
+          (on0 : Env Term := $on0) (on1 : Term → Env Term := $on1)
+        : Env Term :=
+          if terms.size = 0 then on0
+          else if h : terms.size = 1 then on1 terms[0]
+          else lift% mkTerm $kind terms
+      )
+    | _ => Lean.Macro.throwUnsupported
+  else return mainDefs
+
+/-- Binary equality. -/
+def_2nary% equal := .EQUAL, (mkBool true, pure)
+/-- Binary pairwise inequality. -/
+def_2nary% distinct := .DISTINCT
+
+/-- Logical negation. -/
+def not (boolTerm : Term) := liftKind% .NOT boolTerm
+
+/-- Binary implication. -/
+def_2nary% implies := .IMPLIES
+/-- Binary conjunction. -/
+def_2nary% and := .AND, (mkBool true, pure)
+/-- Binary disjunction. -/
+def_2nary% or := .OR, (mkBool false, pure)
+/-- Binary exclusive-disjunction. -/
+def_2nary% xor := .XOR, (mkBool false, pure)
+
+/-- If-then-else from condition/then-branch/else-branch. -/
+def ite (cnd thn els : Term) := liftKind% .ITE cnd thn els
+@[inherit_doc ite]
+def thenElse := @ite
+
+/-- Binary less-than operator. -/
+def_2nary% lt := .LT
+/-- Binary less-than-or-equal-to operator. -/
+def_2nary% le := .LEQ
+/-- Binary greater-than-or-equal-to operator. -/
+def_2nary% ge := .GEQ
+/-- Binary greater-than operator. -/
+def_2nary% gt := .GT
+
+
+
+/-! ### Arithmetic operators -/
+
+/-- Arithmetic negation. -/
+def neg (arith_term : Term) := liftKind% .NEG arith_term
+
+/-- Binary addition. -/
+def_2nary% add := .ADD, (mkInt 0, pure)
+
+/-- Binary subtraction. -/
+def_2nary% sub := .SUB
+
+/-- Binary multiplication. -/
+def_2nary% mul := .MULT, (mkInt 1, pure)
+
+/-- Binary division over reals, division by `0` undefined, left associative. -/
+def_2nary% real_div := .DIVISION
+/-- Binary division over reals, division by `0` defined to be `0`, left associative. -/
+def_2nary% real_div_total := .DIVISION_TOTAL
+
+/-- Binary division over integers, division by `0` undefined, left associative. -/
+def_2nary% int_div := .INTS_DIVISION
+/-- Binary division over integers, division by `0` defined to be `0`, left associative. -/
+def_2nary% int_div_total := .INTS_DIVISION_TOTAL
+
+/-- Integer modulus, modulus by `0` undefined. -/
+def_2nary% mod := .INTS_MODULUS
+
+/-- Integer modulus, modulus by `0` defined to be `0`. -/
+def_2nary% mod_total := .INTS_MODULUS_TOTAL
+
+/-- Absolute value over arithmetic terms. -/
+def abs (arith_term : Term) := liftKind% .ABS arith_term
+
+/-- Arithmetic power; both terms must have the same sort: either `Int` or `Real`. -/
+def pow (term exp : Term) := liftKind% .POW term exp
+
+/-- Exponential over reals. -/
+def exp (term : Term) := liftKind% .EXPONENTIAL term
+
+
+
+-- /-! ### Array operators -/
+
+/-- The array `a` where `a[i] = if i = idx then elm else array[i]`. -/
+def store (array idx elm : Term) := liftKind% .STORE array idx elm
+
+/-- The element associated with `idx` in `array`. -/
+def select (array idx : Term) := liftKind% .SELECT array idx
+
+
+
+/-! ## String operators -/
+
+def stringConcat (str1 str2 : Term) := liftKind% .STRING_CONCAT str1 str2
+
+def stringConcatN (strings : Terms)
+: (at_least_2 : 1 < strings.size := by grind) → Env Term := fun _ => do
+  runUnsafe fun tm => tm.mkTerm .STRING_CONCAT strings
+
+def stringLength (str : Term) := liftKind% .STRING_LENGTH str
+
+
+
+/-! ## Substitution -/
+
+/-- Term substitution specification. -/
+structure Subst where
+/-- Creates a `∀ i, terms[i] ↦ replacements[i]` substitution. -/
+mk ::
+  /-- Terms to replace. -/
+  ts : Terms
+  /-- Terms to replace `ts` elements by. -/
+  rs : Terms
+  /-- Proof that they have the same size. -/
+  same_size : ts.size = rs.size := by
+    (try assumption) <;> (try grind) <;> fail "failed to prove term arrays have the same size"
+
+namespace Subst
+
+/-- A function taking a proof that both term arrays have the same size and producing `β`. -/
+abbrev SameSize (ts1 ts2 : Terms) (β : Type) :=
+  (same_size : ts1.size = ts2.size :=
+    by (try assumption) <;> (try grind) <;> fail "failed to prove term arrays have the same size")
+  → β
+
+/-- Creates a `term ↦ replacement` substitution. -/
+def mkOne (term : Term) (replacement : Term) : Subst := mk #[term] #[replacement]
+
+/-- The empty substitution. -/
+def empty : Subst := {ts := #[], rs := #[], same_size := rfl}
+
+/-- Adds a `term ↦ replacement` substitution. -/
+def push (s : Subst) (term : Term) (replacement : Term) : Subst := {s with
+  ts := s.ts.push term
+  rs := s.rs.push replacement
+  same_size := by grind only [!Array.size_push, s.same_size]
+}
+
+/-- Augments a substitution with `∀ i, terms[i] ↦ replacements[i]`. -/
+def extend (s : Subst)
+  (terms : Terms) (replacements : Terms)
+: SameSize terms replacements Subst := fun same_size => {s with
+  ts := s.ts.append terms
+  rs := s.rs.append replacements
+  same_size := by
+    simp only [Array.append_eq_append, Array.size_append, s.same_size, Nat.add_left_cancel_iff]
+    assumption
+}
+
+end Subst
+
+@[inherit_doc T.substitute]
+def substitute (term : Term) (subst : Subst) : Env Term :=
+  runUnsafe' do T.substitute term subst.ts subst.rs
+
+
+
+/-! ### Accessors -/
+
+/-- The `Kind` of a term. -/
+def getKind (term : Term) : Res Kind := T.getKind term
+
+/-- The sub-terms of a term. -/
+def getKids (term : Term) : Array Term := term.getChildren
+
+/-- Size-checked sub-terms of a term. -/
+def getSizedKids (term : Term) (size : Nat) : Env {array : Array Term // array.size = size} := do
+  let kids := term.getKids
+  if h : kids.size = size then return ⟨kids, h⟩ else
+    throwUser s!"expected {size} kid(s), got {kids.size} in term `{term}` of kind {term.getKind?}"
+
+@[inherit_doc T.getSort]
+def getSort (term : Term) : Env Srt := do
+  let srt ← T.getSort term |>.mapError Error.ofUnsafe
+  return by unfold Srt ; exact srt
+
+
+-- /-! ### Value extraction -/
+
+@[inherit_doc T.isBooleanValue]
+def isBoolValue (term : Term) : Bool := T.isBooleanValue term
+/-- If `term` is a boolean value, produces that value; fails otherwise. -/
+def getBoolValue (term : Term) : Res Bool := T.getBooleanValue term |>.mapError Error.ofUnsafe
+/-- If `term` is a boolean value, produces that value. -/
+def getBoolValue? (term : Term) : Option Bool := T.getBooleanValue? term
+
+@[inherit_doc T.isIntegerValue]
+def isIntValue (term : Term) : Bool := T.isIntegerValue term
+/-- If `term` is an integer value, produces that value; fails otherwise. -/
+def getIntValue (term : Term) : Res Int := T.getIntegerValue term |>.mapError Error.ofUnsafe
+/-- If `term` is an integer value, produces that value. -/
+def getIntValue? (term : Term) : Option Int := T.getIntegerValue? term
+
+@[inherit_doc T.isRealValue]
+def isRealValue (term : Term) : Bool := T.isRealValue term
+/-- If `term` is a real value, produces that value as a string; fails otherwise. -/
+def getRealValue (term : Term) : Res String := T.getRealValue term |>.mapError Error.ofUnsafe
+/-- If `term` is a real value, produces that value as a string. -/
+def getRealValue? (term : Term) : Option String := T.getRealValue? term
+/-- If `term` is a real value, produces that value as a `Rat`; fails otherwise. -/
+def getRatValue (term : Term) : Res Rat := T.getRationalValue term |>.mapError Error.ofUnsafe
+/-- If `term` is a real value, produces that value as a `Rat`. -/
+def getRatValue? (term : Term) : Option Rat := T.getRationalValue? term
+
+@[inherit_doc T.isStringValue]
+def isStringValue (term : Term) : Bool := T.isStringValue term
+/-- If `term` is an integer value, produces that value; fails otherwise. -/
+def getStringValue (term : Term) : Res String :=
+  if term.isStringValue then
+    let s := term.toString
+    if s.startsWith '"' ∧ s.endsWith '"' then return s.drop 1 |>.dropEnd 1 |>.toString
+    else throwUser s!"failed to retrieve string value of term `{s}`"
+  else throwUser "cannot extract string-value of of a non-string-value term"
+/-- If `term` is an integer value, produces that value. -/
+def getStringValue? (term : Term) : Option String := term.getStringValue.toOption
+
+def getRegexValue (term : Term) : Env Regex :=
+  throwTodo s!"regex value extraction from a constant term: {term}"
+
+def getRoundingModeValue (term : Term) : Env Float.RoundingMode :=
+  throwTodo s!"rounding mode value extraction from a constant term: {term}"
+
+def getSeqValue [A : TermToValue α] (t : Term) : Env (Array α) := do
+  let elms ← t.getSequenceValue |>.mapError Error.ofUnsafe
+  elms.mapM getValue
+
+def getSeqValueOf (α : Type) [A : TermToValue α] : (t : Term) → Env (Array α) := getSeqValue
+
+def getBitVecValue (t : Term) : Env (BitVec size) := do
+  let binRepr ← t.getBitVectorValue 2 |>.mapError Error.ofUnsafe
+  let empty : (size : Nat) × BitVec size := ⟨0, BitVec.zero 0⟩
+  let ⟨size', bv⟩ ← binRepr.chars.foldM (init := empty) fun
+    | ⟨size, bv⟩, '0' => pure ⟨size + 1, bv.concat false⟩
+    | ⟨size, bv⟩, '1' => pure ⟨size + 1, bv.concat true⟩
+    | _, c => throwInternal
+      s!"unexpected character `{c}` in binary representation `{binRepr}` for bitvec term `{t}`"
+  if h : size' = size
+  then return h ▸ bv
+  else throwUser s!"expected bitvector term of size {size}, got size {size'}: {t}"
+
+
+instance : SrtLike Bool where
+  termToValue t := t.getBoolValue
+  valueToTerm := mkBool
+
+instance : SrtLike Int where
+  termToValue t := t.getIntValue
+  valueToTerm := mkInt
+
+instance : ValueToTerm Nat where
+  valueToTerm n := mkInt n
+
+instance : SrtLike Rat where
+  termToValue t := t.getRatValue
+  valueToTerm := mkReal
+
+instance : SrtLike String where
+  termToValue t := t.getStringValue
+  valueToTerm := mkString
+
+instance : SrtLike Regex where
+  termToValue t := t.getRegexValue
+  valueToTerm _value := throwTodo s!"value-to-term for `Regex`"
+
+instance : SrtLike Float.RoundingMode where
+  termToValue t := t.getRoundingModeValue
+  valueToTerm := mkRoundingMode
+
+instance : SrtLike (BitVec size) where
+  termToValue t := t.getBitVecValue
+  valueToTerm := mkBitVec
+
+section variable [ToTyp α]
+
+instance [TermToValue α] : TermToValue (Array α) := ⟨getSeqValue⟩
+
+instance [ValueToTerm α] : ValueToTerm (Array α) := ⟨mkSeqValue⟩
+end
