Cvc/Untyped/Types/Bag.lean
@@ -1,0 +1,87 @@
+module
+
+import all Cvc.Untyped.Srt
+
+public import Cvc.Untyped.Term
+public import Std.Data.TreeMap.Basic
+
+
+
+namespace Cvc public section variable [Ω]
+
+open Untyped
+
+abbrev Bag (α : Type) [Ord α] := Std.TreeMap α Int
+
+namespace Bag variable [Ord α] (bag : Bag α)
+
+def empty : Bag α := Std.TreeMap.empty
+
+def alter (key : α) (f : Int → Int) : Bag α :=
+  Std.TreeMap.alter bag key fun val? => match val?.getD 0 |> f with | 0 => none | n => n
+
+def increment (key : α) := bag.alter key (· + 1)
+
+def decrement (key : α) := bag.alter key (· - 1)
+
+def add (key : α) (n : Int) := bag.alter key (· + n)
+
+def sub (key : α) (n : Int) := bag.alter key (· - n)
+
+def get? (key : α) : Option Int := Std.TreeMap.get? bag key
+
+def get (key : α) : Int := bag.get? key |>.getD 0
+
+def contains (key : α) : Bool := 0 < bag.get key
+
+protected abbrev mem (key : α) : Prop := bag.contains key
+
+instance : Membership α (Bag α) := ⟨Bag.mem⟩
+
+omit [Ω] in
+theorem mem_def {key : α} : (key ∈ bag) = bag.contains key := rfl
+
+instance (key : α) : Decidable (key ∈ bag) :=
+  bag.mem_def ▸ if h : bag.contains key then isTrue h else isFalse h
+
+protected def toString [ToString α] (bag : Bag α) : String :=
+  bag.foldl (init := "") fun
+    | acc, _key, 0 => acc
+    | acc, key, n => s!"{if acc.isEmpty then acc else acc ++ ", "}{key} ↦ {n}"
+
+instance [ToString α] : ToString (Bag α) := ⟨Bag.toString⟩
+
+instance [A : ToTyp α] : ToTyp (Bag α) := ⟨.bag A.typ⟩
+
+section variable [A : ToTyp α] [Ord α]
+
+def toTerm [ValueToTerm α] (set : Bag α) : Env Term := do
+  let empty ← Srt.of (Bag α) >>= Term.mkEmptyBag
+  set.foldlM (init := empty) fun bag elem count => do
+    let elem ← Term.mkValue elem
+    let count ← Term.mkInt count
+    Term.mkBagWith elem count >>= bag.bagUnionMax
+
+instance [ValueToTerm α] : ValueToTerm (Bag α) := ⟨toTerm⟩
+
+partial def ofTerm [TermToValue α] (t : Term) : Env (Bag α) := do
+  let k ← t.getKind
+  match k with
+  | .BAG_EMPTY => return Bag.empty
+  | .BAG_MAKE =>
+    let ⟨kids, _⟩ ← t.getSizedKids 2
+    let elem ← Term.getValue kids[0]
+    let count ← Term.getValue kids[1]
+    return Bag.empty.insert elem count
+  | .BAG_UNION_MAX
+  | .BAG_UNION_DISJOINT
+  | .BAG_INTER_MIN
+  | .BAG_DIFFERENCE_SUBTRACT
+  | .BAG_DIFFERENCE_REMOVE => throwTodo s!"bag-value reconstruction for term-kind `{k}`"
+  | _ => throwUser s!"expected `{A.typ}`-bag"
+
+instance [TermToValue α] : TermToValue (Bag α) := ⟨ofTerm⟩
+
+end
+
+end Bag
