Cvc/Untyped/Types/FiniteField.lean
@@ -1,0 +1,73 @@
+module
+
+import all Cvc.Basic.Env
+import all Cvc.Untyped.Srt
+
+public import Cvc.Untyped.Term
+
+
+
+namespace Cvc public section variable [Ω]
+
+open Untyped
+
+/-- An element of a finite field of size `size`. -/
+structure FiniteField (size : Nat) where
+  /-- Element representation. -/
+  repr : Int
+deriving DecidableEq, Hashable, Ord
+
+namespace FiniteField
+
+instance : ToTyp (FiniteField size) := ⟨.finiteField size⟩
+
+/-- Erased version of `FiniteField`. -/
+structure Erased where
+  /-- The field's size. -/
+  size : Nat
+  /-- The actual finite field element. -/
+  get : FiniteField size
+
+/-- Erases a finite-field-element's size. -/
+def erase (elem : FiniteField size) : Erased := {size, get := elem}
+
+/-- String representation. -/
+protected def toString (ff : FiniteField size) : String := toString ff.repr
+
+instance : ToString (FiniteField size) := ⟨FiniteField.toString⟩
+
+/-- Creates a constant finite-field-element term. -/
+def toTerm (elem : FiniteField size) : Env Term :=
+  Srt.of (FiniteField size) >>= Term.mkFiniteFieldElemOfValue elem.repr
+
+namespace Erased
+@[inherit_doc FiniteField.toString]
+protected def toString (elem : Erased) := elem.get.toString
+
+instance : ToString Erased := ⟨Erased.toString⟩
+
+@[inherit_doc FiniteField.toTerm]
+def toTerm (elem : Erased) : Env Term := elem.get.toTerm
+
+/-- Retrieves the value of a constant finite-field-element term. -/
+def ofTerm (t : Term) : Env Erased := do
+  let srt ← t.getSort
+  let size ← srt.getFiniteFieldSize
+  let ff ← t.getFiniteFieldValue
+  return {size, get := {repr := ff}}
+
+instance : TermToValue Erased := ⟨ofTerm⟩
+instance : ValueToTerm Erased := ⟨toTerm⟩
+end Erased
+
+/-- Retrieves the `FiniteField` value of a constant finite-field-element term. -/
+def ofTerm (t : Term) : Env (FiniteField size) := do
+  let ⟨size', elem⟩ ← Erased.ofTerm t
+  if h : size' = size then return h ▸ elem
+  else throwUser s!"expected finite-field-element of size {size}, got one of size {size'}: {t}"
+
+instance : SrtLike (FiniteField size) where
+  termToValue := ofTerm
+  valueToTerm := toTerm
+
+end FiniteField
