Cvc/Untyped/Types/Set.lean
@@ -1,0 +1,57 @@
+module
+
+import all Cvc.Basic.Env
+import all Cvc.Untyped.Srt
+
+public import Cvc.Untyped.Term
+public import Std.Data.TreeSet.Basic
+
+
+
+namespace Cvc public section variable [Ω]
+
+open Untyped
+
+/-- Alias for `Std.TreeSet`. -/
+abbrev Set (α : Type) [Ord α] := Std.TreeSet α
+
+namespace Set variable [Ord α]
+
+open Std renaming TreeSet → S
+
+@[inherit_doc S.empty] def empty : Set α := S.empty
+@[inherit_doc S.ofArray] def ofArray := S.ofArray (α := α)
+
+instance [A : ToTyp α] : ToTyp (Set α) := ⟨.set A.typ⟩
+
+/-- String representation. -/
+protected def toString [ToString α] (set : Set α) : String :=
+  if set.isEmpty then "∅" else Id.run do
+    let mut s := ""
+    let mut sep := ""
+    for elem in set do
+      s := s!"{s}{sep}{elem}"
+      sep := ", "
+    s!"\{ {s} }"
+
+instance [ToString α] : ToString (Set α) := ⟨Set.toString⟩
+
+section variable [ToTyp α] [Ord α]
+
+def toTerm [ValueToTerm α] (set : Set α) : Env Term := do
+  let mut term ← Srt.of (Set α) >>= Term.mkEmptySet
+  for elem in set do
+    term ← Term.mkValue elem >>= term.setInsert
+  return term
+
+instance [ValueToTerm α] : ValueToTerm (Set α) := ⟨toTerm⟩
+
+def ofTerm [TermToValue α] (t : Term) : Env (Set α) := do
+  let elems ← t.getSetValue
+  elems.foldlM (init := Set.empty) fun set term => set.insert <$> Term.getValue term
+
+instance [TermToValue α] : TermToValue (Set α) := ⟨ofTerm⟩
+
+end
+
+end Set
